Current state

Simple_Clause_Learning/Simple_Clause_Learning.thy
@@ -38,6 +38,9 @@ subsection \<open>Set_Extra\<close>
 lemma not_in_iff: "L \<notin> xs \<longleftrightarrow> (\<forall>y\<in>xs. L \<noteq> y)"
   by auto
 
+lemma disjoint_iff': "A \<inter> B = {} \<longleftrightarrow> (\<forall>a \<in> A. a \<notin> B) \<and> (\<forall>b \<in> B. b \<notin> A)"
+  by blast
+
 
 subsection \<open>List_Extra\<close>
 
@@ -171,6 +174,102 @@ subsection \<open>First_Order_Terms Extra\<close>
 
 
 subsubsection \<open>First_Order_Terms Only\<close>
+
+lemma atm_of_eq_uminus_if_lit_eq: "L = - K \<Longrightarrow> atm_of L = atm_of K"
+  by (cases L; cases K) simp_all
+
+term subst_domain
+
+lemma mem_range_varsI:
+  assumes "\<sigma> x = Var y" "x \<noteq> y"
+  shows "y \<in> range_vars \<sigma>"
+  unfolding range_vars_def UN_iff
+proof (rule bexI[of _ "Var y"])
+  show "y \<in> vars_term (Var y)" by simp
+next
+  from assms show "Var y \<in> subst_range \<sigma>"
+    by (simp_all add: subst_domain_def)
+qed
+
+lemma subst_apply_term_eq_subst_apply_term_composeI:
+  assumes
+    "range_vars \<sigma> \<inter> subst_domain \<delta> = {}"
+    "x \<notin> subst_domain \<delta>"
+  shows "\<sigma> x = (\<sigma> \<circ>\<^sub>s \<delta>) x"
+proof (cases "\<sigma> x")
+  case (Var y)
+  show ?thesis
+  proof (cases "x = y")
+    case True
+    with Var have \<open>\<sigma> x = Var x\<close> by simp
+    moreover from \<open>x \<notin> subst_domain \<delta>\<close> have "\<delta> x = Var x"
+      by (simp add: disjoint_iff subst_domain_def)
+    ultimately show ?thesis
+      by (simp add: subst_compose_def)
+  next
+    case False
+    with Var have "y \<in> range_vars \<sigma>"
+      by (auto intro: mem_range_varsI)
+    hence "y \<notin> subst_domain \<delta>"
+      using \<open>range_vars \<sigma> \<inter> subst_domain \<delta> = {}\<close>
+      by (simp add: disjoint_iff)
+    with Var show ?thesis
+      unfolding subst_compose_def
+      by (simp add: subst_domain_def)
+  qed
+next
+  case (Fun f ys)
+  hence "Fun f ys \<in> subst_range \<sigma> \<or> (\<forall>y\<in>set ys. y \<in> subst_range \<sigma>)"
+    using subst_domain_def by fastforce
+  hence " \<forall>x\<in>vars_term (Fun f ys). x \<in> range_vars \<sigma>"
+    by (metis UN_I range_vars_def term.distinct(1) term.sel(4) term.set_cases(2))
+  hence "Fun f ys \<cdot> \<delta> = Fun f ys \<cdot> Var"
+    unfolding term_subst_eq_conv
+    using \<open>range_vars \<sigma> \<inter> subst_domain \<delta> = {}\<close>
+    by (simp add: disjoint_iff subst_domain_def)
+  hence "Fun f ys \<cdot> \<delta> = Fun f ys"
+    by simp
+  with Fun show ?thesis
+    by (simp add: subst_compose_def)
+qed
+
+lemma subst_comp_in_unifiersI:
+  assumes "t \<cdot> \<sigma> = u \<cdot> \<delta>" and
+    "vars_term t \<inter> subst_domain \<delta> = {}" and
+    "vars_term u \<inter> subst_domain \<sigma> = {}" and
+    "range_vars \<sigma> \<inter> subst_domain \<delta> = {}"
+  shows "\<sigma> \<circ>\<^sub>s \<delta> \<in> unifiers {(t, u)}"
+proof -
+  have "t \<cdot> \<sigma> = t \<cdot> \<sigma> \<cdot> \<delta>"
+    unfolding term_subst_eq_conv[of t \<sigma> "\<sigma> \<circ>\<^sub>s \<delta>", simplified]
+    using \<open>vars_term t \<inter> subst_domain \<delta> = {}\<close> \<open>range_vars \<sigma> \<inter> subst_domain \<delta> = {}\<close>
+    by (auto intro: subst_apply_term_eq_subst_apply_term_composeI)
+  moreover have "u \<cdot> \<delta> = u \<cdot> \<sigma> \<cdot> \<delta>"
+    unfolding term_subst_eq_conv[of u \<delta> "\<sigma> \<circ>\<^sub>s \<delta>", simplified]
+    using \<open>vars_term u \<inter> subst_domain \<sigma> = {}\<close>
+    by (simp add: disjoint_iff subst_compose_def subst_domain_def)
+  ultimately show ?thesis
+    using \<open>t \<cdot> \<sigma> = u \<cdot> \<delta>\<close> by (simp add: unifiers_def)
+qed
+
+lemma subst_comp_in_unifiersI':
+  assumes "t \<cdot> \<sigma> = u \<cdot> \<delta>" and
+    "vars_term t \<inter> subst_domain \<delta> = {}" and
+    "vars_term u \<inter> subst_domain \<sigma> = {}" and
+    "range_vars \<delta> \<inter> subst_domain \<sigma> = {}"
+  shows "\<delta> \<circ>\<^sub>s \<sigma> \<in> unifiers {(t, u)}"
+proof -
+  have "t \<cdot> \<sigma> = t \<cdot> \<delta> \<cdot> \<sigma>"
+    unfolding term_subst_eq_conv[of t \<sigma> "\<delta> \<circ>\<^sub>s \<sigma>", simplified]
+    using \<open>vars_term t \<inter> subst_domain \<delta> = {}\<close>
+    by (simp add: disjoint_iff subst_compose_def subst_domain_def)
+  moreover have "u \<cdot> \<delta> = u \<cdot> \<delta> \<cdot> \<sigma>"
+    unfolding term_subst_eq_conv[of u \<delta> "\<delta> \<circ>\<^sub>s \<sigma>", simplified]
+    using \<open>vars_term u \<inter> subst_domain \<sigma> = {}\<close> \<open>range_vars \<delta> \<inter> subst_domain \<sigma> = {}\<close>
+    by (auto intro: subst_apply_term_eq_subst_apply_term_composeI)
+  ultimately show ?thesis
+    using \<open>t \<cdot> \<sigma> = u \<cdot> \<delta>\<close> by (simp add: unifiers_def)
+qed
 
 lemma mgu_ball_codom_is_Var:
   assumes mgu_\<mu>: "is_mgu \<mu> E"
@@ -326,6 +425,114 @@ proof -
     by (metis (mono_tags, lifting) multiset.set_map set_mset_mset vars_mset_def)
 qed
 
+lemma subst_ident_if_not_in_domain: "x \<notin> subst_domain \<mu> \<Longrightarrow> \<mu> x = Var x"
+  by (simp add: subst_domain_def)
+
+lemma
+  assumes mgu_\<mu>: "is_imgu \<mu> {(t, u)}" and ren_\<rho>: "is_renaming \<rho>" and inj_\<rho>: "inj \<rho>"
+  defines "\<mu>' \<equiv> (\<lambda>x.
+    if x \<in> the_Var ` \<rho> ` subst_domain \<mu> then
+      ((Var o the_inv \<rho>) \<circ>\<^sub>s \<mu> \<circ>\<^sub>s \<rho>) (Var x)
+    else
+      Var x)"
+  shows "is_imgu \<mu>' {(t \<cdot> \<rho>, u \<cdot> \<rho>)}"
+proof (unfold is_imgu_def, intro conjI ballI)
+  have *: "t \<cdot> \<rho> \<cdot> \<mu>' = t \<cdot> \<mu> \<cdot> \<rho>" for t
+    unfolding subst_subst
+  proof (rule term_subst_eq)
+    fix x
+    assume "x \<in> vars_term t"
+    obtain x' where "\<rho> x = Var x'"
+      using ren_\<rho> by (meson is_Var_def is_renaming_def)
+    hence inv_\<rho>_x': "the_inv \<rho> (Var x') = x"
+      using inj_\<rho> by (metis the_inv_f_f)
+      
+    show "(\<rho> \<circ>\<^sub>s \<mu>') x = (\<mu> \<circ>\<^sub>s \<rho>) x"
+    proof (cases "x \<in> subst_domain \<mu>")
+      case True
+      hence "x' \<in> the_Var ` \<rho> ` subst_domain \<mu>"
+        using \<open>\<rho> x = Var x'\<close> by (metis imageI term.sel(1))
+      then show ?thesis
+        by (simp add: \<open>\<rho> x = Var x'\<close> \<mu>'_def subst_compose_def inv_\<rho>_x')
+    next
+      case False
+      moreover hence "x' \<notin> the_Var ` \<rho> ` subst_domain \<mu>"
+        by (smt (verit, best) \<open>\<rho> x = Var x'\<close> image_iff inj_\<rho> inj_image_mem_iff is_renaming_def ren_\<rho>
+            term.collapse(1))
+      ultimately show ?thesis
+        by (simp add: subst_compose_def subst_ident_if_not_in_domain[of x \<mu>] \<mu>'_def \<open>\<rho> x = Var x'\<close>)
+    qed
+  qed
+
+  from mgu_\<mu> have "t \<cdot> \<mu> = u \<cdot> \<mu>"
+    using is_imgu_def by fastforce
+  then show "\<mu>' \<in> unifiers {(t \<cdot> \<rho>, u \<cdot> \<rho>)}"
+    unfolding unifiers_def mem_Collect_eq
+    by (simp add: *)
+next
+  fix \<upsilon>
+  assume "\<upsilon> \<in> unifiers {(t \<cdot> \<rho>, u \<cdot> \<rho>)}"
+  hence "t \<cdot> \<rho> \<cdot> \<upsilon> = u \<cdot> \<rho> \<cdot> \<upsilon>"
+    by fastforce
+
+  with mgu_\<mu> have "\<rho> \<circ>\<^sub>s \<upsilon> = \<mu> \<circ>\<^sub>s \<rho> \<circ>\<^sub>s \<upsilon>"
+    unfolding is_imgu_def
+    by (simp add: subst_monoid_mult.mult_assoc unifiers_insert)
+
+  show "\<upsilon> = \<mu>' \<circ>\<^sub>s \<upsilon>"
+  proof (rule ext)
+    fix x
+    show "\<upsilon> x = (\<mu>' \<circ>\<^sub>s \<upsilon>) x"
+      apply (cases " x \<in> the_Var ` \<rho> ` subst_domain \<mu>")
+      apply (simp_all add: \<mu>'_def subst_compose_def)
+      using \<open>\<rho> \<circ>\<^sub>s \<upsilon> = \<mu> \<circ>\<^sub>s \<rho> \<circ>\<^sub>s \<upsilon>\<close>
+      by (smt (verit, del_insts) imageE inj_\<rho> is_renaming_def ren_\<rho> subst_compose
+          subst_monoid_mult.mult.left_neutral term.collapse(1) the_inv_f_f)
+  qed
+qed
+
+(* lemma fixes \<upsilon> :: "'a \<Rightarrow> ('b, 'a) Term.term" assumes "\<upsilon> \<in> unifiers E" shows "\<exists>\<mu>. is_mgu \<mu> E"
+  unfolding is_mgu_def
+proof (rule ccontr)
+  assume "\<nexists>\<mu>. \<mu> \<in> unifiers E \<and> (\<forall>\<tau>\<in>unifiers E. \<exists>\<gamma>. \<tau> = \<mu> \<circ>\<^sub>s \<gamma>)"
+  fix epred5_5 :: "('b, 'a) Term.term set \<Rightarrow> ('a \<Rightarrow> ('b, 'a) Term.term) \<Rightarrow> ('b, 'a) Term.term set \<Rightarrow> ('a \<Rightarrow> ('b, 'a) Term.term) \<Rightarrow>  ('b, 'a) Term.term set \<Rightarrow> bool"
+  have "\<And>(X1 :: 'a \<Rightarrow> ('b, 'a) Term.term) (X2 :: ('b, 'a) Term.term set)
+    (X3 :: 'a \<Rightarrow> ('b, 'a) Term.term)  (X4 :: ('b, 'a) Term.term set) (X5 :: ('b, 'a) Term.term set).
+    epred5_5 X5 X3 X4 X1 X2 \<longleftrightarrow> \<not> (X3 \<in> X4 \<longrightarrow> True)"
+(* thf(c_0_5, plain,
+![X1:a > term_b_a, X2:set_a_term_b_a, X3:a > term_b_a, X4:set_a_term_b_a, X5:set_a_term_b_a]:
+  (((epred5_5 @ X5 @ X3 @ X4 @ X1 @ X2)<=>
+  (~(member_a_term_b_a @ X3 @ X4)=>
+    (((insert_a_term_b_a @ X1 @ X2)=(insert_a_term_b_a @ X3 @ X4))<=>
+      ((((X1)!=(X3))|(((X2)=(X4))))&
+        (((X1)=(X3))|((~((((X2)=(insert_a_term_b_a @ X3 @ X5))&
+          (~(member_a_term_b_a @ X3 @ X5)&
+          (((X4)=(insert_a_term_b_a @ X1 @ X5))&~(member_a_term_b_a @ X1 @ X5)))))
+          |(?[X5:set_a_term_b_a]:($true)))&
+      ((((X2)=(insert_a_term_b_a @ X3 @ X5))&
+      (~(member_a_term_b_a @ X3 @ X5)&
+        (((X4)=(insert_a_term_b_a @ X1 @ X5))&~(member_a_term_b_a @ X1 @ X5))))|
+        (?[X5:set_a_term_b_a]:($false)))))))))), introduced(definition)). *)
+  show False
+  using insert_eq_iff mk_disjoint_insert subst_monoid_mult.mult.right_neutral
+  (* sledgehammer [e, slices = 1, dont_minimize, isar_proof, compress = 1, timeout = 30, preplay_timeout = 10, overlord] (insert_eq_iff mk_disjoint_insert subst_monoid_mult.mult.right_neutral) *)
+  (* by (metis insert_eq_iff mk_disjoint_insert subst_monoid_mult.mult.right_neutral) *)
+  using ex_in_conv insertI1 insert_absorb insert_commute insert_eq_iff insert_iff
+    insert_not_empty is_mgu_def mk_disjoint_insert subst_monoid_mult.mult.right_neutral
+  (* by (smt (verit) ex_in_conv insertI1 insert_absorb insert_commute insert_eq_iff insert_iff
+      insert_not_empty is_mgu_def mk_disjoint_insert subst_monoid_mult.mult.right_neutral) *) *)
+
+lemma "is_renaming (Var(x := Var x'))"
+proof (unfold is_renaming_def, intro conjI allI)
+  fix y show "is_Var ((Var(x := Var x')) y)"
+    by simp
+next
+  show "inj_on (Var(x := Var x')) (subst_domain (Var(x := Var x')))"
+    apply (rule inj_onI)
+    apply (simp add: subst_domain_def)
+    by presburger
+qed
+
 
 subsubsection \<open>First_Order_Terms And Abstract_Substitution\<close>
 
@@ -364,6 +571,12 @@ lemma vars_cls_plus_iff: "vars_cls (C + D) = vars_cls C \<union> vars_cls D"
 lemma is_ground_atm_iff_vars_empty: "is_ground_atm t \<longleftrightarrow> vars_term t = {}"
   by (metis (mono_tags, opaque_lifting) equals0D equals0I is_ground_atm_def subst_apply_term_empty
       subst_def subst_simps(1) term.distinct(1) term_subst_eq term_subst_eq_rev)
+
+lemma is_ground_lit_iff_vars_empty: "is_ground_lit L \<longleftrightarrow> vars_lit L = {}"
+  by (simp add: is_ground_atm_iff_vars_empty is_ground_lit_def)
+
+lemma is_ground_cls_iff_vars_empty: "is_ground_cls C \<longleftrightarrow> vars_cls C = {}"
+  by (auto simp: is_ground_cls_def is_ground_lit_iff_vars_empty vars_cls_def)
 
 lemma is_ground_atm_is_ground_on_var:
   assumes "is_ground_atm (A \<cdot>a \<sigma>)" and "v \<in> vars_term A"
@@ -678,6 +891,9 @@ lemma subst_lit_idem_if_disj_vars: "subst_domain \<sigma> \<inter> vars_lit L = 
 definition restrict_subst where
   "restrict_subst V \<sigma> x \<equiv> (if x \<in> V then \<sigma> x else Var x)"
 
+lemma restrict_subst_empty[simp]: "restrict_subst {} \<sigma> = Var"
+  unfolding restrict_subst_def by auto
+
 lemma subst_domain_restrict_subst: "subst_domain (restrict_subst V \<sigma>) \<subseteq> V"
   unfolding restrict_subst_def subst_domain_def
   by auto
@@ -763,6 +979,9 @@ lemma range_vars_renaming_subset_domain_inv:
 definition rename_clause ::
   "('f, 'a) term clause set \<Rightarrow> ('f, 'a) term clause \<Rightarrow> ('f, 'a) term clause" where
   "rename_clause N C = C \<cdot> renaming_wrt N"
+
+lemma rename_clause_mempty[simp]: "rename_clause N {#} = {#}"
+  by (simp add: rename_clause_def)
 
 lemma disjoint_vars_set_insert_rename_clause:
   assumes fin_N: "finite N" and disj_N: "disjoint_vars_set N"
@@ -856,6 +1075,10 @@ definition trail_propagate ::
     ('f, 'v) trail" where
   "trail_propagate \<Gamma> L C \<gamma> = (L \<cdot>l \<gamma>, Some (C, L, \<gamma>)) # \<Gamma>"
 
+lemma suffix_trail_propagate[simp]: "suffix \<Gamma> (trail_propagate \<Gamma> L C \<delta>)"
+  unfolding suffix_def trail_propagate_def
+  by simp
+
 lemma clss_of_trail_trail_propagate[simp]:
   "clss_of_trail (trail_propagate \<Gamma> L C \<gamma>) = clss_of_trail \<Gamma> \<union> {C + {#L#}}"
   unfolding trail_propagate_def clss_of_trail_def by simp
@@ -941,8 +1164,16 @@ lemma trail_backtrack_level_eq:
   "level \<le> trail_level \<Gamma> \<Longrightarrow> trail_level (trail_backtrack \<Gamma> level) = level"
   by (induction \<Gamma>) auto
 
+lemma trail_backtrack_propagate[simp]:
+  "trail_backtrack (trail_propagate \<Gamma> L C \<gamma>) n = trail_backtrack \<Gamma> n"
+  by (simp add: trail_propagate_def is_decision_lit_def)
+
 definition trail_interp :: "('f, 'v) trail \<Rightarrow> ('f, 'v) term interp" where
   "trail_interp \<Gamma> = \<Union>((\<lambda>L. case L of Pos A \<Rightarrow> {A} | Neg A \<Rightarrow> {}) ` fst ` set \<Gamma>)"
+
+primrec trail_grounding :: "('f, 'v) trail \<Rightarrow> ('f, 'v) subst" where
+  "trail_grounding [] = (Var :: ('f, 'v) subst)" |
+  "trail_grounding (Ln # \<Gamma>) = (case snd Ln of None \<Rightarrow> Var | Some _ \<Rightarrow> Var) \<odot> trail_grounding \<Gamma>"
 
 definition trail_true_lit :: "('f, 'v) trail \<Rightarrow> ('f, 'v) term literal \<Rightarrow> bool" where
   "trail_true_lit \<Gamma> L \<longleftrightarrow> L \<in> fst ` set \<Gamma>"
@@ -962,15 +1193,36 @@ definition trail_true_clss :: "('f, 'v) trail \<Rightarrow> ('f, 'v) term clause
 definition trail_defined_lit :: "('f, 'v) trail \<Rightarrow> ('f, 'v) term literal \<Rightarrow> bool" where
   "trail_defined_lit \<Gamma> L \<longleftrightarrow> (L \<in> fst ` set \<Gamma> \<or> - L \<in> fst ` set \<Gamma>)"
 
+definition trail_defined_cls :: "('f, 'v) trail \<Rightarrow> ('f, 'v) term clause \<Rightarrow> bool" where
+  "trail_defined_cls \<Gamma> C \<longleftrightarrow> (\<forall>L \<in># C. trail_defined_lit \<Gamma> L)"
+
 lemma trail_defined_lit_iff_true_or_false:
   "trail_defined_lit \<Gamma> L \<longleftrightarrow> trail_true_lit \<Gamma> L \<or> trail_false_lit \<Gamma> L"
   unfolding trail_defined_lit_def trail_false_lit_def trail_true_lit_def by (rule refl)
+
+lemma trail_false_cls_mempty[simp]: "trail_false_cls \<Gamma> {#}"
+  by (simp add: trail_false_cls_def)
+
+lemma not_trail_true_Nil[simp]:
+  "\<not> trail_true_lit [] L"
+  "\<not> trail_true_cls [] C"
+  "N \<noteq> {} \<Longrightarrow> \<not> trail_true_clss [] N"
+  by (simp_all add: trail_true_lit_def trail_true_cls_def trail_true_clss_def)
+
+lemma not_trail_false_Nil[simp]:
+  "\<not> trail_false_lit [] L"
+  "C \<noteq> {#} \<Longrightarrow> \<not> trail_false_cls [] C"
+  by (simp_all add: trail_false_lit_def trail_false_cls_def)
 
 lemma ball_trail_backtrackI:
   assumes "\<forall>x \<in> set \<Gamma>. P (fst x)"
   shows "\<forall>x \<in> set (trail_backtrack \<Gamma> i). P (fst x)"
   using assms trail_backtrack_suffix[THEN set_mono_suffix]
   by blast
+
+lemma trail_false_lit_if_trail_false_suffix:
+  "suffix \<Gamma>' \<Gamma> \<Longrightarrow> trail_false_lit \<Gamma>' K \<Longrightarrow> trail_false_lit \<Gamma> K"
+  by (meson image_mono set_mono_suffix subsetD trail_false_lit_def)
 
 lemma trail_interp_Cons: "trail_interp (Ln # \<Gamma>) = trail_interp [Ln] \<union> trail_interp \<Gamma>"
   unfolding trail_interp_def by simp
@@ -1011,6 +1263,32 @@ lemma ball_trail_decide_is_ground_lit:
   unfolding trail_decide_def
   using assms
   by simp
+
+lemma trail_false_cls_subst_mgu_before_grounding:
+  assumes tr_false_cls: "trail_false_cls \<Gamma> ((D + {#L, L'#}) \<cdot> \<sigma>)" and
+    mgu_L_L': "Unifiers.is_imgu \<mu> {(atm_of L, atm_of L')}" and
+    \<sigma>_unif: "\<sigma> \<in> Unifiers.unifiers {(atm_of L, atm_of L')}"
+  shows "trail_false_cls \<Gamma> ((D + {#L#}) \<cdot> \<mu> \<cdot> \<sigma>)"
+  unfolding trail_false_cls_def
+proof (rule ballI)
+  fix K
+  assume "K \<in># (D + {#L#}) \<cdot> \<mu> \<cdot> \<sigma>"
+  hence "K \<in># D \<cdot> \<mu> \<cdot> \<sigma> \<or> K = L  \<cdot>l \<mu> \<cdot>l \<sigma>" by force
+  thus "trail_false_lit \<Gamma> K"
+  proof (elim disjE)
+    show "K \<in># D \<cdot> \<mu> \<cdot> \<sigma> \<Longrightarrow> trail_false_lit \<Gamma> K"
+      using mgu_L_L' \<sigma>_unif
+      by (metis Unifiers.is_imgu_def subst_cls_comp_subst subst_cls_union tr_false_cls
+          trail_false_cls_def union_iff)
+  next
+    have "L \<cdot>l \<mu> \<cdot>l \<sigma> = L \<cdot>l \<sigma>"
+      using mgu_L_L' \<sigma>_unif
+      unfolding Unifiers.is_imgu_def
+      by (metis subst_lit_comp_subst)
+    thus "K = L \<cdot>l \<mu> \<cdot>l \<sigma> \<Longrightarrow> trail_false_lit \<Gamma> K"
+      by (auto intro: tr_false_cls[unfolded trail_false_cls_def, rule_format])
+  qed
+qed
 
 
 section \<open>SCL Calculus\<close>
@@ -1201,6 +1479,15 @@ next
       by (cases u) auto
   qed (use Cons in simp_all)
 qed
+
+lemma ball_ground_lit_if_sound_trail: "sound_trail N U \<Gamma> \<Longrightarrow> \<forall>L \<in> fst ` set \<Gamma>. is_ground_lit L"
+proof (induction \<Gamma> rule: sound_trail.induct)
+  case Nil
+  show ?case by simp
+next
+  case (Cons \<Gamma> L u)
+  thus ?case by auto
+qed 
 
 lemma sound_trail_backtrackI: "sound_trail N U \<Gamma> \<Longrightarrow> sound_trail N U (trail_backtrack \<Gamma> level)"
   by (induction \<Gamma> rule: sound_trail.induct) (auto intro: sound_trail.intros)
@@ -1422,30 +1709,11 @@ proof (induction S S' rule: factorize.induct)
 
   moreover have "trail_false_cls \<Gamma> ((D + {#L#}) \<cdot> \<mu> \<cdot> \<sigma>')"
   proof -
-    have "trail_false_cls \<Gamma> ((D + {#L#}) \<cdot> \<mu> \<cdot> \<sigma>)"
-      unfolding trail_false_cls_def
-    proof (rule ballI)
-      fix K
-      assume "K \<in># (D + {#L#}) \<cdot> \<mu> \<cdot> \<sigma>"
-      hence "K \<in># D \<cdot> \<mu> \<cdot> \<sigma> \<or> K = L  \<cdot>l \<mu> \<cdot>l \<sigma>" by force
-      thus "trail_false_lit \<Gamma> K"
-      proof (elim disjE)
-        show "K \<in># D \<cdot> \<mu> \<cdot> \<sigma> \<Longrightarrow> trail_false_lit \<Gamma> K"
-          apply (rule tr_false_cls[unfolded trail_false_cls_def, rule_format])
-          using is_imgu_\<mu>_full \<sigma>_unif_full
-          by (metis (no_types, lifting) Unifiers.is_imgu_def subst_cls_comp_subst subst_cls_union
-              union_iff)
-      next
-        have "L \<cdot>l \<mu> \<cdot>l \<sigma> = L \<cdot>l \<sigma>"
-          using mgu_sound[OF mgu_L_L'] \<sigma>_unif
-          unfolding Unifiers.is_imgu_def
-          by (metis subst_lit_comp_subst)
-        thus "K = L \<cdot>l \<mu> \<cdot>l \<sigma> \<Longrightarrow> trail_false_lit \<Gamma> K"
-          by (auto intro: tr_false_cls[unfolded trail_false_cls_def, rule_format])
-      qed
-    qed
-    thus ?thesis
-      unfolding \<sigma>'_def using subst_cls_restrict_subst_idem by (metis subsetI)
+    show ?thesis
+      unfolding \<sigma>'_def
+      using subst_cls_restrict_subst_idem
+      using trail_false_cls_subst_mgu_before_grounding[OF tr_false_cls mgu_sound[OF mgu_L_L'] \<sigma>_unif]
+      by (metis subsetI)
   qed
 
   moreover have "N \<TTurnstile>\<G>e {(D + {#L#}) \<cdot> \<mu>}"
@@ -1471,6 +1739,53 @@ proof (induction S S' rule: factorize.induct)
   ultimately show ?case
     unfolding sound_state_def
     using fin_N fin_U disj_N_U sound_\<Gamma> N_entails_U by simp
+qed
+
+
+lemma trail_false_cls_plus_subst_mgu_before_groundings:
+  assumes
+    tr_false_\<Gamma>_D_L'_\<sigma>: "trail_false_cls \<Gamma> ((D + {#L'#}) \<cdot> \<sigma>)" and
+    tr_false_\<Gamma>'_C_\<delta>: "trail_false_cls \<Gamma>' (C \<cdot> \<delta>)" and
+    "suffix \<Gamma>' \<Gamma>" and
+    gr_D_L'_\<sigma>: "is_ground_cls ((D + {#L'#}) \<cdot> \<sigma>)" and
+    vars_D_L'_vars_C_L_disj: "vars_cls (D + {#L'#}) \<inter> vars_cls (C + {#L#}) = {}" and
+    dom_\<sigma>: "subst_domain \<sigma> \<subseteq> vars_cls (D + {#L'#})" and
+    is_imgu_\<mu>: "Unifiers.is_imgu \<mu> {(atm_of L, atm_of L')}" and
+    \<sigma>_\<delta>_in_unif: "\<sigma> \<odot> \<delta> \<in> unifiers {(atm_of L, atm_of L')}"
+  shows "trail_false_cls \<Gamma> ((D + C) \<cdot> \<mu> \<cdot> \<sigma> \<cdot> \<delta>)"
+  unfolding subst_cls_union trail_false_cls_def
+proof (rule ballI)
+  fix K
+  assume "K \<in># D \<cdot> \<mu> \<cdot> \<sigma> \<cdot> \<delta> + C \<cdot> \<mu> \<cdot> \<sigma> \<cdot> \<delta>"
+  thus "trail_false_lit \<Gamma> K"
+    unfolding union_iff
+  proof (elim disjE)
+    assume K_in: "K \<in># D \<cdot> \<mu> \<cdot> \<sigma> \<cdot> \<delta>"
+    hence "K \<in># D \<cdot> \<sigma> \<cdot> \<delta>"
+      using is_imgu_\<mu> \<sigma>_\<delta>_in_unif
+      by (metis Unifiers.is_imgu_def subst_cls_comp_subst)
+    hence "K \<in># D \<cdot> \<sigma>"
+      using gr_D_L'_\<sigma> is_ground_subst_cls by (metis is_ground_cls_union subst_cls_union)
+    then show ?thesis
+      by (auto intro!: tr_false_\<Gamma>_D_L'_\<sigma>[unfolded trail_false_cls_def, rule_format])
+  next
+    assume "K \<in># C \<cdot> \<mu> \<cdot> \<sigma> \<cdot> \<delta>"
+    hence "K \<in># C \<cdot> \<sigma> \<cdot> \<delta>"
+      using is_imgu_\<mu> \<sigma>_\<delta>_in_unif
+      by (metis Unifiers.is_imgu_def subst_cls_comp_subst)
+    have "K \<in># C \<cdot> \<delta>"
+    proof -
+      have "subst_domain \<sigma> \<inter> vars_cls C = {}"
+        using dom_\<sigma> vars_D_L'_vars_C_L_disj
+        by auto
+      thus ?thesis
+        using \<open>K \<in># C \<cdot> \<sigma> \<cdot> \<delta>\<close> subst_cls_idem_if_disj_vars[of \<sigma> C] by simp
+    qed
+    hence tr_false_\<Gamma>'_K:"trail_false_lit \<Gamma>' K"
+      using tr_false_\<Gamma>'_C_\<delta>[unfolded trail_false_cls_def, rule_format, of K] by simp
+    show ?thesis
+      by (rule trail_false_lit_if_trail_false_suffix[OF \<open>suffix \<Gamma>' \<Gamma>\<close> tr_false_\<Gamma>'_K])
+  qed
 qed
 
 lemma resolve_sound_state: "resolve N S S' \<Longrightarrow> sound_state N S \<Longrightarrow> sound_state N S'"
@@ -1515,24 +1830,24 @@ proof (induction S S' rule: resolve.induct)
     unfolding \<Gamma>_def trail_propagate_def
     by auto
 
-  have is_imgu_\<mu>_full:
-    "Unifiers.is_imgu \<mu> (insert (atm_of L, atm_of L') ((\<lambda>t. (t, t)) ` atm_of ` set_mset (C + D)))"
-    using mgu_sound[OF mgu_L_L']
-    by (smt (verit, best) Unifiers.is_imgu_def imageE insert_iff mem_Collect_eq prod.sel singletonD
-        unifiers_def)
-
-  from L_eq_comp_L' have "L \<cdot>l \<sigma> \<cdot>l \<delta> = - (L' \<cdot>l \<sigma> \<cdot>l \<delta>)"
-    using dom_\<sigma> dom_\<delta>
-    using subst_lit_idem_if_disj_vars[of \<sigma> L]
-    by (smt (verit) Un_Int_eq(4) add_mset_eq_single gr_D_L'_\<sigma> inf.commute inf.orderE inf_bot_right
-        inf_sup_aci(2) is_ground_cls_union is_ground_subst_cls subst_cls_single subst_cls_union
-        sup_bot.right_neutral vars_D_L'_vars_C_L_disj vars_cls_add_mset vars_cls_empty
-        vars_cls_plus_iff)
-
-  hence \<sigma>_\<delta>_in_unif:"\<sigma> \<odot> \<delta> \<in> unifiers
-    (insert (atm_of L, atm_of L') ((\<lambda>t. (t, t)) ` atm_of ` set_mset (C + D)))"
-    unfolding unifiers_def mem_Collect_eq
-    by (auto intro: subst_atm_of_eq_compI[of _ "\<sigma> \<odot> \<delta>", simplified])
+  have \<sigma>_\<delta>_in_unif: "\<sigma> \<odot> \<delta> \<in> unifiers {(atm_of L, atm_of L')}"
+  proof (rule subst_comp_in_unifiersI')
+    show "atm_of L \<cdot>a \<delta> = atm_of L' \<cdot>a \<sigma>"
+      using L_eq_comp_L' by (metis atm_of_eq_uminus_if_lit_eq atm_of_subst_lit)
+  next
+    show "vars_lit L \<inter> subst_domain \<sigma> = {}"
+      using dom_\<sigma> vars_D_L'_vars_C_L_disj by auto
+  next
+    show "vars_lit L' \<inter> subst_domain \<delta> = {}"
+      using dom_\<delta> vars_D_L'_vars_C_L_disj by auto
+  next
+    have "range_vars \<sigma> = {}"
+      unfolding range_vars_def UNION_empty_conv subst_range.simps
+      using dom_\<sigma> gr_D_L'_\<sigma> is_ground_cls_is_ground_on_var is_ground_atm_iff_vars_empty
+      by fast
+    thus "range_vars \<sigma> \<inter> subst_domain \<delta> = {}"
+      by simp
+  qed
 
   have "disjoint_vars ((D + C) \<cdot> \<mu> \<cdot> \<rho>) E" if E_in: "E \<in> N \<union> U \<union> clss_of_trail \<Gamma>" for E
   proof -
@@ -1579,7 +1894,7 @@ proof (induction S S' rule: resolve.induct)
     from gr_D_L'_\<sigma> have "is_ground_cls ((D + {#L'#}) \<cdot> \<sigma> \<cdot> \<delta>)"
       by (metis is_ground_subst_cls)
     hence "is_ground_cls ((D + {#L'#}) \<cdot> \<mu> \<cdot> \<sigma> \<cdot> \<delta>)"
-      by (metis (no_types, lifting) Unifiers.is_imgu_def \<sigma>_\<delta>_in_unif is_imgu_\<mu>_full
+      by (metis (no_types, lifting) Unifiers.is_imgu_def \<sigma>_\<delta>_in_unif mgu_sound[OF mgu_L_L']
           subst_cls_comp_subst)
     thus "is_ground_cls (D \<cdot> \<mu> \<cdot> \<sigma> \<cdot> \<delta>)"
       by (metis is_ground_cls_union subst_cls_union)
@@ -1589,7 +1904,7 @@ proof (induction S S' rule: resolve.induct)
       using dom_\<sigma> vars_D_L'_vars_C_L_disj
       by (smt (verit, best) Int_assoc inf.orderE inf_bot_right subst_cls_idem_if_disj_vars)
     hence "is_ground_cls ((C + {#L#}) \<cdot> \<mu> \<cdot> \<sigma> \<cdot> \<delta>)"
-      by (metis (no_types, lifting) Unifiers.is_imgu_def \<sigma>_\<delta>_in_unif is_imgu_\<mu>_full
+      by (metis (no_types, lifting) Unifiers.is_imgu_def \<sigma>_\<delta>_in_unif mgu_sound[OF mgu_L_L']
           subst_cls_comp_subst)
     thus "is_ground_cls (C \<cdot> \<mu> \<cdot> \<sigma> \<cdot> \<delta>)"
       by (metis is_ground_cls_union subst_cls_union)
@@ -1599,71 +1914,18 @@ proof (induction S S' rule: resolve.induct)
     ((D + C) \<cdot> \<mu> \<cdot> \<rho> \<cdot> restrict_subst (vars_cls ((D + C) \<cdot> \<mu> \<cdot> \<rho>)) (inv_renaming' \<rho> \<odot> \<sigma> \<odot> \<delta>))"
     unfolding subst_cls_restrict_subst_idem[OF subset_refl]
     unfolding subst_cls_comp_subst subst_cls_renaming_inv_renaming_idem[OF is_renaming_\<rho>]
-    unfolding subst_cls_union trail_false_cls_def
-  proof (rule ballI)
-    fix K
-    assume "K \<in># D \<cdot> \<mu> \<cdot> \<sigma> \<cdot> \<delta> + C \<cdot> \<mu> \<cdot> \<sigma> \<cdot> \<delta>"
-    thus "trail_false_lit \<Gamma> K"
-      unfolding union_iff
-    proof (elim disjE)
-      assume K_in: "K \<in># D \<cdot> \<mu> \<cdot> \<sigma> \<cdot> \<delta>"
-      hence "K \<in># D \<cdot> \<sigma> \<cdot> \<delta>"
-        using is_imgu_\<mu>_full[unfolded Unifiers.is_imgu_def, THEN conjunct2, rule_format,
-            OF \<sigma>_\<delta>_in_unif]
-        by (metis subst_cls_comp_subst)
-      hence "K \<in># D \<cdot> \<sigma>"
-        using gr_D_L'_\<sigma> is_ground_subst_cls by (metis is_ground_cls_union subst_cls_union)
-      then show ?thesis
-        by (auto intro!: tr_false_cls[unfolded trail_false_cls_def, rule_format])
-    next
-      have tr_false_cls_C: "trail_false_cls \<Gamma>' (C \<cdot> \<delta>)"
-        using sound_\<Gamma>
-        unfolding sound_trail.simps[of _ _ \<Gamma>]
-        unfolding \<Gamma>_def trail_propagate_def
-        by simp
+  proof -
+    have tr_false_cls_C: "trail_false_cls \<Gamma>' (C \<cdot> \<delta>)"
+      using sound_\<Gamma>
+      unfolding sound_trail.simps[of _ _ \<Gamma>]
+      unfolding \<Gamma>_def trail_propagate_def
+      by simp
 
-      assume "K \<in># C \<cdot> \<mu> \<cdot> \<sigma> \<cdot> \<delta>"
-      hence "K \<in># C \<cdot> \<sigma> \<cdot> \<delta>"
-        using is_imgu_\<mu>_full[unfolded Unifiers.is_imgu_def, THEN conjunct2, rule_format,
-            OF \<sigma>_\<delta>_in_unif]
-        by (metis subst_cls_comp_subst)
-      have "K \<in># C \<cdot> \<delta>"
-      proof -
-        have "subst_domain \<sigma> \<inter> vars_cls C = {}"
-          using dom_\<sigma> vars_D_L'_vars_C_L_disj
-          by auto
-        thus ?thesis
-          using \<open>K \<in># C \<cdot> \<sigma> \<cdot> \<delta>\<close> subst_cls_idem_if_disj_vars[of \<sigma> C] by simp
-      qed
-      hence tr_false_\<Gamma>'_K:"trail_false_lit \<Gamma>' K"
-        using tr_false_cls_C[unfolded trail_false_cls_def, rule_format, of K] by simp
-      show ?thesis
-      proof (cases "L \<cdot>l \<delta>")
-        case L_Pos: (Pos t)
-        show ?thesis
-        proof (cases K)
-          case K_Pos: (Pos u)
-          then show ?thesis
-            using L_Pos tr_false_\<Gamma>'_K tr_undef_\<Gamma>'_L_\<delta>
-            unfolding \<Gamma>_def trail_false_lit_def trail_propagate_def trail_defined_lit_def
-              trail_true_lit_def trail_interp_Cons'
-            by simp
-        next
-          case (Neg u)
-          then show ?thesis
-            using L_Pos tr_false_\<Gamma>'_K
-            unfolding \<Gamma>_def trail_false_lit_def trail_propagate_def
-            unfolding trail_interp_Cons' prod.sel
-            by simp
-        qed
-      next
-        case (Neg t)
-        then show ?thesis
-          using tr_false_\<Gamma>'_K
-          unfolding \<Gamma>_def trail_false_lit_def trail_propagate_def
-          unfolding trail_interp_Cons' prod.sel
-          by simp
-      qed
+    show "trail_false_cls \<Gamma> ((D + C) \<cdot> \<mu> \<cdot> \<sigma> \<cdot> \<delta>)"
+    proof (rule trail_false_cls_plus_subst_mgu_before_groundings[OF tr_false_cls tr_false_cls_C _
+          gr_D_L'_\<sigma> vars_D_L'_vars_C_L_disj dom_\<sigma> mgu_sound[OF mgu_L_L'] \<sigma>_\<delta>_in_unif])
+      show "suffix \<Gamma>' \<Gamma>"
+        by (simp add: \<Gamma>_def suffix_ConsI trail_propagate_def)
     qed
   qed
 
@@ -1795,6 +2057,40 @@ theorem scl_sound_state:
     factorize_sound_state resolve_sound_state backtrack_sound_state
   by metis
 
+lemma assumes "sound_state N S" and "conflict N S S'"
+  shows "(\<exists>\<gamma>. state_conflict S' = Some ({#}, \<gamma>)) \<or> (\<exists>S''. backtrack N S' S'')"
+proof -
+  from \<open>conflict N S S'\<close> obtain D U D' \<Gamma> \<sigma> where
+       "S = (\<Gamma>, U, None)" and
+       S'_def: "S' = (\<Gamma>, U, Some (D', \<sigma>))" and
+       "D \<in> N \<union> U"
+       "D' = rename_clause (N \<union> U \<union> clss_of_trail \<Gamma>) D"
+       "subst_domain \<sigma> \<subseteq> vars_cls D'"
+       "is_ground_cls (D' \<cdot> \<sigma>)"
+       "trail_false_cls \<Gamma> (D' \<cdot> \<sigma>)"
+    by (auto elim: conflict.cases)
+
+  then show ?thesis
+  proof (cases "D' = {#}")
+    assume "D' = {#}"
+    with S'_def show ?thesis by simp
+  next
+    assume "D' \<noteq> {#}"
+    then obtain D'' L where "D' = D'' + {#L#}"
+      by (metis add_mset_add_single multi_nonempty_split)
+    have "(\<exists>S''. backtrack N S' S'')"
+      unfolding S'_def \<open>D' = D'' + {#L#}\<close>
+    proof (rule exI)
+      show "backtrack N (\<Gamma>, U, Some (D'' + {#L#}, \<sigma>))
+        (trail_backtrack \<Gamma> (trail_level_cls \<Gamma> (D'' \<cdot> \<sigma>)), U \<union> {D'' + {#L#}}, None)"
+        apply (rule backtrackI)
+        
+        sorry
+    qed
+    thus ?thesis ..
+  qed
+  oops
+
 
 section \<open>Reasonable And Regular Runs\<close>
 
@@ -1807,9 +2103,463 @@ lemma scl_if_reasonable: "reasonable_scl N S S' \<Longrightarrow> scl N S S'"
 definition regular_scl where
   "regular_scl N S S' \<longleftrightarrow> conflict N S S' \<or> \<not> conflict N S S' \<and> reasonable_scl N S S'"
 
+context
+  fixes a b c d e f g :: "('f, 'v) term"
+  assumes distinct_terms: "distinct [a, b, c, d, e, f, g]" and
+    ball_is_ground_atm: "\<forall>t \<in> {a, b, c, d, e, f, g}. is_ground_atm t"
+begin
+
+definition C1 where
+  "C1 = {#Neg a, Pos b#}"
+
+definition C2 where
+  "C2 = {#Neg a, Pos c#}"
+
+definition C3 where
+  "C3 = {#Neg b, Pos d#}"
+
+definition C4 where
+  "C4 = {#Neg c, Neg d#}"
+
+definition C5 where
+  "C5 = {#Pos e, Pos f, Pos g#}"
+
+definition N where
+  "N = {C1, C2, C3, C4, C5}"
+
+
+lemma ball_is_ground_cls: "\<forall>C \<in> N. is_ground_cls C"
+  using ball_is_ground_atm
+  by (simp add: N_def C1_def C2_def C3_def C4_def C5_def is_ground_cls_def is_ground_lit_def)
+
+lemma rename_clause_ident_if_ground[simp]:
+  fixes N C
+  shows "is_ground_cls C \<Longrightarrow> rename_clause N C = C"
+  by (simp add: rename_clause_def)
+
+lemma is_ground_lit_Pos[simp]: "is_ground_atm L \<Longrightarrow> is_ground_lit (Pos L)"
+  by (simp add: is_ground_lit_def)
+
+lemma is_ground_lit_Neg[simp]: "is_ground_atm L \<Longrightarrow> is_ground_lit (Neg L)"
+  by (simp add: is_ground_lit_def)
+
+
+definition S1 where
+  "S1 = ([(Pos a, None)], {}, None)"
+
+lemma "regular_scl N initial_state S1"
+proof (unfold regular_scl_def, rule disjI2, rule conjI)
+  show "\<not> conflict N initial_state S1"
+    unfolding S1_def
+    by (simp add: conflict.simps)
+next
+  have "decide N initial_state (trail_decide [] (Pos a), {}, None)"
+    by (rule decideI)
+      (simp_all add: ball_is_ground_atm is_ground_lit_def trail_defined_lit_iff_true_or_false)
+  hence "scl N initial_state (trail_decide [] (Pos a), {}, None)"
+    by (simp add: scl_def)
+  moreover have "\<nexists>S. conflict N (trail_decide [] (Pos a), {}, None) S"
+    apply (rule notI)
+    apply (elim exE conflict.cases)
+    using ball_is_ground_cls distinct_terms
+    by (auto simp: N_def C1_def C2_def C3_def C4_def C5_def
+        trail_decide_def trail_false_cls_def trail_false_lit_def)
+  ultimately show "reasonable_scl N initial_state S1"
+    unfolding reasonable_scl_def by (simp add: S1_def trail_decide_def)
+qed
+
+
+definition S2 where
+  "S2 = ([
+    (Pos e, None),
+    (Pos a, None)], {}, None)"
+
+lemma "regular_scl N S1 S2"
+proof (unfold regular_scl_def, rule disjI2, rule conjI)
+  show "\<not> conflict N S1 S2"
+    unfolding S1_def S2_def
+    by (simp add: conflict.simps)
+next
+  have "decide N S1 S2"
+    unfolding S1_def S2_def
+    using distinct_terms ball_is_ground_atm
+    by (auto simp: decide.simps trail_decide_def trail_defined_lit_def)
+  hence "scl N S1 S2"
+    unfolding scl_def by simp
+  moreover have "\<nexists>S. conflict N S2 S"
+    apply (rule notI)
+    apply (elim exE conflict.cases)
+    using ball_is_ground_cls distinct_terms
+    by (auto simp add: N_def S2_def C1_def C2_def C3_def C4_def C5_def trail_false_cls_def
+        trail_false_lit_def)
+  ultimately show "reasonable_scl N S1 S2"
+    unfolding reasonable_scl_def by simp
+qed
+
+
+definition S3 :: "('f, 'v) state" where
+  "S3 = ([
+    (Pos b, Some ({#Neg a#}, Pos b, Var)),
+    (Pos e, None),
+    (Pos a, None)], {}, None)"
+
+lemma "regular_scl N S2 S3"
+proof (unfold regular_scl_def, rule disjI2, rule conjI)
+  show "\<not> conflict N S2 S3"
+    unfolding S2_def S3_def
+    by (simp add: conflict.simps)
+next
+  have "propagate N S2 S3"
+    unfolding S2_def S3_def
+    unfolding propagate.simps
+    apply (rule exI[of _ C1])
+    using distinct_terms ball_is_ground_cls ball_is_ground_atm
+    by (auto simp add: N_def C1_def trail_propagate_def is_ground_cls_def trail_false_cls_def
+        trail_false_lit_def trail_defined_lit_def)
+  hence "scl N S2 S3"
+    unfolding scl_def by simp
+  moreover have "\<nexists>S. conflict N S3 S"
+    apply (rule notI)
+    apply (elim exE conflict.cases)
+    using ball_is_ground_cls distinct_terms
+    by (auto simp add: N_def S3_def C1_def C2_def C3_def C4_def C5_def trail_false_cls_def
+        trail_false_lit_def)
+  ultimately show "reasonable_scl N S2 S3"
+    unfolding reasonable_scl_def by simp
+qed
+
+
+definition S4 :: "('f, 'v) state" where
+  "S4 = ([
+    (Pos c, Some ({#Neg a#}, Pos c, Var)),
+    (Pos b, Some ({#Neg a#}, Pos b, Var)),
+    (Pos e, None),
+    (Pos a, None)], {}, None)"
+
+lemma "regular_scl N S3 S4"
+proof (unfold regular_scl_def, rule disjI2, rule conjI)
+  show "\<not> conflict N S3 S4"
+    unfolding S3_def S4_def
+    by (simp add: conflict.simps)
+next
+  have "propagate N S3 S4"
+    unfolding S3_def S4_def
+    unfolding propagate.simps
+    apply (rule exI[of _ C2])
+    using distinct_terms ball_is_ground_cls ball_is_ground_atm
+    by (auto simp add: N_def C2_def trail_propagate_def is_ground_cls_def trail_false_cls_def
+        trail_false_lit_def trail_defined_lit_def)
+  hence "scl N S3 S4"
+    unfolding scl_def by simp
+  moreover have "decide N S3 S4 \<Longrightarrow> \<nexists>S. conflict N S4 S"
+    using \<open>propagate N S3 S4\<close> decide_well_defined(1) by blast
+  ultimately show "reasonable_scl N S3 S4"
+    unfolding reasonable_scl_def by simp
+qed
+
+
+definition S5 :: "('f, 'v) state" where
+  "S5 = ([
+    (Pos d, Some ({#Neg b#}, Pos d, Var)),
+    (Pos c, Some ({#Neg a#}, Pos c, Var)),
+    (Pos b, Some ({#Neg a#}, Pos b, Var)),
+    (Pos e, None),
+    (Pos a, None)], {}, None)"
+
+lemma "regular_scl N S4 S5"
+proof (unfold regular_scl_def, rule disjI2, rule conjI)
+  show "\<not> conflict N S4 S5"
+    unfolding S4_def S5_def
+    by (simp add: conflict.simps)
+next
+  have "propagate N S4 S5"
+    unfolding S4_def S5_def
+    unfolding propagate.simps
+    apply (rule exI[of _ C3])
+    using distinct_terms ball_is_ground_cls ball_is_ground_atm
+    by (auto simp add: N_def C3_def trail_propagate_def is_ground_cls_def trail_false_cls_def
+        trail_false_lit_def trail_defined_lit_def)
+  hence "scl N S4 S5"
+    unfolding scl_def by simp
+  moreover have "decide N S4 S5 \<Longrightarrow> \<nexists>S. conflict N S5 S"
+    using \<open>propagate N S4 S5\<close> decide_well_defined(1) by blast
+  ultimately show "reasonable_scl N S4 S5"
+    unfolding reasonable_scl_def by simp
+qed
+
+
+definition S6 :: "('f, 'v) state" where
+  "S6 = ([
+    (Pos d, Some ({#Neg b#}, Pos d, Var)),
+    (Pos c, Some ({#Neg a#}, Pos c, Var)),
+    (Pos b, Some ({#Neg a#}, Pos b, Var)),
+    (Pos e, None),
+    (Pos a, None)], {}, Some (C4, Var))"
+
+lemma "regular_scl N S5 S6"
+proof (unfold regular_scl_def, rule disjI1)
+  show "conflict N S5 S6"
+    unfolding S5_def S6_def
+    using ball_is_ground_cls
+    apply (simp add: conflict.simps N_def)
+    apply (rule exI[of _ C4])
+    by (simp add: C4_def trail_false_cls_def trail_false_lit_def)
+qed
+
+lemma zip_option_same: "zip_option xs xs = Some (zip xs xs)"
+  by (induction xs)  (simp_all add: zip_option.simps)
+
+lemma decompose_same:
+  "\<And>f. decompose (Fun f ss) (Fun f ss) = Some (zip ss ss)"
+  by (simp add: decompose_def zip_option_same)
+
+lemma unify_append_eq_unify_if_prefix_same: "(\<forall>e \<in> set es1. fst e = snd e) \<Longrightarrow> unify (es1 @ es2) bs = unify es2 bs"
+proof (induction "es1 @ es2" bs arbitrary: es1 es2 bs rule: unify.induct)
+  case (1 bs)
+  thus ?case by simp
+next
+  case (2 f ss g ts E bs)
+  show ?case
+  proof (cases es1)
+    case Nil
+    thus ?thesis by simp
+  next
+    case (Cons e es1')
+    hence e_def: "e = (Fun f ss, Fun g ts)" and E_def: "E = es1' @ es2"
+      using "2" by simp_all
+    hence "f = g" and "ss = ts"
+      using "2.prems" local.Cons by auto
+    then show ?thesis
+      apply (simp add: Cons e_def decompose_same)
+      apply (rule "2"(1)[of _ "zip ts ts @ es1'" es2, simplified])
+      apply simp
+        apply (rule decompose_same)
+      unfolding E_def apply simp
+      by (metis "2.prems" UnE in_set_zip list.set_intros(2) local.Cons)
+    qed
+next
+  case (3 x t E bs)
+  show ?case
+  proof (cases es1)
+    case Nil
+    thus ?thesis by simp
+  next
+    case (Cons e es1')
+    hence e_def: "e = (Var x, t)" and E_def: "E = es1' @ es2"
+      using 3 by simp_all
+    show ?thesis
+    proof (cases "t = Var x")
+      case True
+      show ?thesis
+        using 3(1)[OF True E_def]
+        using "3.hyps"(3) "3.prems" local.Cons by fastforce
+    next
+      case False
+      then show ?thesis
+        using "3.prems" e_def local.Cons by force
+    qed
+  qed
+next
+  case (4 v va x E bs)
+  then show ?case
+  proof (cases es1)
+    case Nil
+    thus ?thesis by simp
+  next
+    case (Cons e es1')
+    hence e_def: "e = (Fun v va, Var x)" and E_def: "E = es1' @ es2"
+      using 4 by simp_all
+    then show ?thesis
+      using "4.prems" local.Cons by fastforce
+  qed
+qed
+
+
+lemma mgu_same: "Unification.mgu t t = Some Var"
+  unfolding Unification.mgu.simps
+  unfolding unify_append_eq_unify_if_prefix_same[of "[(t, t)]" for t, simplified]
+  by simp
+
+definition S7 :: "('f, 'v) state" where
+  "S7 = ([
+    (Pos d, Some ({#Neg b#}, Pos d, Var)),
+    (Pos c, Some ({#Neg a#}, Pos c, Var)),
+    (Pos b, Some ({#Neg a#}, Pos b, Var)),
+    (Pos e, None),
+    (Pos a, None)], {}, Some ({#Neg c, Neg b#}, Var))"
+
+lemma "regular_scl N S6 S7"
+proof (unfold regular_scl_def, rule disjI2, rule conjI)
+  show "\<not> conflict N S6 S7"
+    unfolding S6_def S7_def
+    by (simp add: conflict.simps)
+next
+  have "resolve N S6 S7"
+    unfolding S6_def S7_def C4_def
+    unfolding resolve.simps
+    apply (rule exI[of _ "state_trail S6"])
+    apply (rule exI[of _ "state_trail S4"])
+    apply (rule exI[of _ "Pos d"])
+    apply (rule exI[of _ "{#Neg b#}"])
+    apply (rule exI[of _ Var])
+    apply (rule exI[of _ "{#Neg c#}"])
+    apply (rule exI[of _ Var])
+    apply (rule exI[of _ "renaming_wrt
+        (N \<union> clss_of_trail (state_trail S6) \<union>
+         {{#Neg c#} + {#Neg d#}})"])
+    apply (rule exI[of _ "{}"])
+    apply (rule exI[of _ "Neg d"])
+    apply (rule exI[of _ Var])
+    apply (intro conjI)
+          apply (simp add: S6_def)
+         apply (simp add: S6_def)
+         apply (rule conjI)
+    using ball_is_ground_atm apply simp
+    using ball_is_ground_atm apply (simp add: is_ground_atm_iff_vars_empty)
+        apply (simp add: S4_def S6_def trail_propagate_def)
+       apply (simp add: S6_def trail_propagate_def is_decision_lit_def trail_level_cls_def)
+      apply simp
+     apply simp
+    by (simp del: Unification.mgu.simps add: mgu_same)
+  hence "scl N S6 S7"
+    unfolding scl_def by simp
+  moreover have "decide N S6 S7 \<Longrightarrow> \<nexists>S. conflict N S7 S"
+    using \<open>resolve N S6 S7\<close> decide_well_defined by blast
+  ultimately show "reasonable_scl N S6 S7"
+    unfolding reasonable_scl_def by simp
+qed
+
+
+definition S8 :: "('f, 'v) state" where
+  "S8 = ([
+    (Pos c, Some ({#Neg a#}, Pos c, Var)),
+    (Pos b, Some ({#Neg a#}, Pos b, Var)),
+    (Pos e, None),
+    (Pos a, None)], {}, Some ({#Neg c, Neg b#}, Var))"
+
+lemma "regular_scl N S7 S8"
+proof (unfold regular_scl_def, rule disjI2, rule conjI)
+  show "\<not> conflict N S7 S8"
+    unfolding S7_def S8_def
+    by (simp add: conflict.simps)
+next
+  have "skip N S7 S8"
+    unfolding S7_def S8_def
+    using distinct_terms
+    by (auto simp add: skip.simps trail_propagate_def)
+  hence "scl N S7 S8"
+    unfolding scl_def by simp
+  moreover have "decide N S7 S8 \<Longrightarrow> \<nexists>S. conflict N S8 S"
+    using \<open>skip N S7 S8\<close> decide_well_defined by blast
+  ultimately show "reasonable_scl N S7 S8"
+    unfolding reasonable_scl_def by simp
+qed
+
+
+definition S9 :: "('f, 'v) state" where
+  "S9 = ([
+    (Pos c, Some ({#Neg a#}, Pos c, Var)),
+    (Pos b, Some ({#Neg a#}, Pos b, Var)),
+    (Pos e, None),
+    (Pos a, None)], {}, Some ({#Neg a, Neg b#}, Var))"
+
+lemma "regular_scl N S8 S9"
+proof (unfold regular_scl_def, rule disjI2, rule conjI)
+  show "\<not> conflict N S8 S9"
+    unfolding S8_def S9_def
+    by (simp add: conflict.simps)
+next
+  have "resolve N S8 S9"
+    unfolding S8_def S9_def
+    unfolding resolve.simps
+    apply (rule exI[of _ "state_trail S4"])
+    apply (rule exI[of _ "state_trail S3"])
+    apply (rule exI[of _ "Pos c"])
+    apply (rule exI[of _ "{#Neg a#}"])
+    apply (rule exI[of _ Var])
+    apply (rule exI[of _ "{#Neg b#}"])
+    apply (rule exI[of _ Var])
+    apply (rule exI[of _ "renaming_wrt
+        (N \<union> clss_of_trail (state_trail S4) \<union>
+         {{#Neg b#} + {#Neg c#}})"])
+    apply (rule exI[of _ "{}"])
+    apply (rule exI[of _ "Neg c"])
+    apply (rule exI[of _ Var])
+    apply (intro conjI)
+          apply (simp add: S4_def)
+    using ball_is_ground_atm apply (simp add: S4_def is_ground_atm_iff_vars_empty)
+    by (simp_all del: Unification.mgu.simps
+          add: S4_def S3_def trail_propagate_def is_decision_lit_def trail_level_cls_def mgu_same
+          is_ground_atm_iff_vars_empty)
+  hence "scl N S8 S9"
+    unfolding scl_def by simp
+  moreover have "decide N S8 S9 \<Longrightarrow> \<nexists>S. conflict N S9 S"
+    using \<open>resolve N S8 S9\<close> decide_well_defined by blast
+  ultimately show "reasonable_scl N S8 S9"
+    unfolding reasonable_scl_def by simp
+qed
+
+
+definition S10 :: "('f, 'v) state" where
+  "S10 = ([
+    (Pos b, Some ({#Neg a#}, Pos b, Var)),
+    (Pos e, None),
+    (Pos a, None)], {}, Some ({#Neg a, Neg b#}, Var))"
+
+lemma "regular_scl N S9 S10"
+proof (unfold regular_scl_def, rule disjI2, rule conjI)
+  show "\<not> conflict N S9 S10"
+    unfolding S9_def S10_def
+    by (simp add: conflict.simps)
+next
+  have "skip N S9 S10"
+    unfolding S9_def S10_def
+    using distinct_terms
+    by (auto simp add: skip.simps trail_propagate_def)
+  hence "scl N S9 S10"
+    unfolding scl_def by simp
+  moreover have "decide N S9 S10 \<Longrightarrow> \<nexists>S. conflict N S10 S"
+    using \<open>skip N S9 S10\<close> decide_well_defined by blast
+  ultimately show "reasonable_scl N S9 S10"
+    unfolding reasonable_scl_def by simp
+qed
+
+
+
+definition S11 :: "('f, 'v) state" where
+  "S11 = ([(Pos a, None)], {{#Neg a, Neg b#}}, None)"
+
+thm N_def[unfolded C1_def C2_def C3_def C4_def C5_def]
+
+lemma "regular_scl N S10 S11"
+proof (unfold regular_scl_def, rule disjI2, rule conjI)
+  show "\<not> conflict N S10 S11"
+    unfolding S10_def S11_def
+    by (simp add: conflict.simps)
+next
+  have "backtrack N S10 S11"
+    unfolding S10_def S11_def
+    unfolding backtrack.simps
+    apply (rule exI[of _ "state_trail S3"])
+    apply (rule exI[of _ "Neg b"])
+    apply (rule exI[of _ Var])
+    apply (rule exI[of _ "{}"])
+    apply (rule exI[of _ "{#Neg a#}"])
+    using distinct_terms
+    by (auto simp add: S3_def is_decision_lit_def trail_level_cls_def)
+  hence "scl N S10 S11"
+    unfolding scl_def by simp
+  moreover have "decide N S10 S11 \<Longrightarrow> \<nexists>S. conflict N S11 S"
+    using \<open>backtrack N S10 S11\<close> decide_well_defined by blast
+  ultimately show "reasonable_scl N S10 S11"
+    unfolding reasonable_scl_def by simp
+qed
+
+end
+
 lemma reasonable_if_regular:
   "regular_scl N S S' \<Longrightarrow> reasonable_scl N S S'"
-  unfolding regular_scl_def (* reasonable_scl_def scl_def *)
+  unfolding regular_scl_def
 proof (elim disjE conjE)
   assume "conflict N S S'"
   hence "scl N S S'"
@@ -1837,6 +2587,108 @@ lemma regular_run_sound_state:
   "(regular_scl N)\<^sup>*\<^sup>* S S' \<Longrightarrow> sound_state N S \<Longrightarrow> sound_state N S'"
   by (smt (verit, best) regular_scl_sound_state rtranclp_induct)
 
+
+lemma assumes "(regular_scl N)\<^sup>*\<^sup>* initial_state S" and "conflict N S S'"
+  shows "\<exists>C \<gamma>. state_conflict S' = Some (C, \<gamma>) \<and>
+    (trail_level_cls (state_trail S) (C \<cdot> \<gamma>) = trail_level (state_trail S))"
+  using \<open>conflict N S S'\<close>
+proof (cases N S S' rule: conflict.cases)
+  case (conflictI D U D' \<Gamma> \<gamma>)
+  show ?thesis
+  proof (intro exI conjI)
+    show "state_conflict S' = Some (D', \<gamma>)"
+      using conflictI by simp
+  next
+    show "trail_level_cls (state_trail S) (D' \<cdot> \<gamma>) = trail_level (state_trail S)"
+    proof (cases "D' \<cdot> \<gamma>")
+      case empty
+      hence "D' = {#}"
+        using subst_cls_empty_iff by blast
+      hence "D = {#}"
+        by (simp add: local.conflictI(4) rename_clause_def)
+      hence "{#} \<in> N \<union> U" 
+        using local.conflictI(3) by force
+      then show ?thesis
+        sorry
+    next
+      case (add x N)
+      then show ?thesis sorry
+    qed
+    oops
+
+lemma
+  assumes "\<forall>C \<in> N. C \<noteq> {#}" and "(regular_scl N)\<^sup>*\<^sup>* initial_state S" and "conflict N S S'"
+  shows "\<exists>\<Gamma> L C \<gamma>. state_trail S = trail_propagate \<Gamma> L C \<gamma>"
+  using assms(2,3)
+proof (induction S rule: rtranclp_induct)
+  case base
+  then obtain D D'  \<sigma> where
+       "D \<in> N" and "D' = rename_clause N D" and "trail_false_cls [] (D' \<cdot> \<sigma>)"
+    by (auto elim: conflict.cases)
+
+  from \<open>\<forall>C \<in> N. C \<noteq> {#}\<close> and \<open>D \<in> N\<close> have "D \<noteq> {#}"
+    by simp
+  hence "D' \<cdot> \<sigma> \<noteq> {#}"
+    by (simp add: \<open>D' = rename_clause N D\<close> rename_clause_def)
+  hence "\<not> trail_false_cls [] (D' \<cdot> \<sigma>)"
+    by (rule not_trail_false_Nil(2))
+  with \<open>trail_false_cls [] (D' \<cdot> \<sigma>)\<close> have False
+    by simp
+  thus ?case ..
+next
+  case (step S S'')
+  from step.hyps have "regular_scl N S S''" by simp
+  with \<open>conflict N S'' S'\<close> have "\<not> conflict N S S''" and "reasonable_scl N S S''"
+    unfolding HOL.atomize_conj
+    by (smt (verit, best) conflict.cases option.distinct(1) prod.inject reasonable_if_regular)
+  hence "scl N S S''" and "decide N S S'' \<longrightarrow> \<not> (\<exists>S'''. conflict N S'' S''')"
+    by (simp_all add: reasonable_scl_def)
+
+  from \<open>scl N S S''\<close> show ?case
+    unfolding scl_def
+  proof (elim disjE)
+    assume "propagate N S S''"
+    thus ?thesis
+      by (elim propagate.cases) auto
+  next
+    assume "decide N S S''"
+    with \<open>conflict N S'' S'\<close> have False
+      using \<open>decide N S S'' \<longrightarrow> \<not> (\<exists>S'''. conflict N S'' S''')\<close> by fast
+    thus ?thesis ..
+  next
+    assume "conflict N S S''"
+    with \<open>\<not> conflict N S S''\<close> have False ..
+    thus ?thesis ..
+  next
+    assume "skip N S S''"
+    with \<open>conflict N S'' S'\<close> have False
+      by (elim skip.cases conflict.cases) simp
+    thus ?thesis ..
+  next
+    assume "factorize N S S''"
+    with \<open>conflict N S'' S'\<close> have False
+      by (elim factorize.cases conflict.cases) simp
+    thus ?thesis ..
+  next
+    assume "resolve N S S''"
+    with \<open>conflict N S'' S'\<close> have False
+      by (elim resolve.cases conflict.cases) simp
+    thus ?thesis ..
+  next
+    assume "backtrack N S S''"
+    then have False
+      apply (elim backtrack.cases)
+      sorry
+    thus ?thesis ..
+  qed
+qed
+
+lemma
+  assumes "(regular_scl N)\<^sup>*\<^sup>* initial_state S" and "conflict N S S'"
+  shows "\<exists>S''. (\<lambda>S S'. skip N S S' \<or> factorize N S S')\<^sup>*\<^sup>* S' S'' \<and> resolve N S S'"
+proof -  
+  oops
+
 lemma not_satisfiable_if_sound_state_conflict_bottom:
   assumes sound_S: "sound_state N S" and conflict_S: "state_conflict S = Some ({#}, \<gamma>)"
   shows "\<not> satisfiable (grounding_of_clss N)"
@@ -1846,8 +2698,286 @@ proof -
   thus ?thesis by simp
 qed
 
+lemma
+  assumes sound: "sound_state N (\<Gamma>, U, Some (C' + {#L#}, \<gamma>))"
+  shows
+    "(\<exists>S'. skip N (\<Gamma>, U, Some (C' + {#L#}, \<gamma>)) S') \<or>
+    (\<exists>S'. factorize N (\<Gamma>, U, Some (C' + {#L#}, \<gamma>)) S') \<or>
+    (\<exists>S'. resolve N (\<Gamma>, U, Some (C' + {#L#}, \<gamma>)) S') \<or>
+    (\<exists>S'. backtrack N (\<Gamma>, U, Some (C' + {#L#}, \<gamma>)) S')"
+proof (cases \<Gamma>)
+  case Nil
+  from sound have "trail_false_cls \<Gamma> ((C' + {#L#}) \<cdot> \<gamma>)"
+    by (simp add: sound_state_def)
+  hence "trail_false_lit \<Gamma> (L \<cdot>l \<gamma>)"
+    by (simp add: trail_false_cls_def)
+  hence False
+    unfolding trail_false_lit_def Nil by simp
+  thus ?thesis
+    by simp
+next
+  case (Cons Ln \<Gamma>')
+  then obtain L n where Ln_def: "Ln = (L, n)" by force
+  show ?thesis
+  proof (cases n)
+    case None
+    show ?thesis
+      unfolding Cons Ln_def None
+      apply (simp add: skip.simps trail_propagate_def resolve.simps)
+      unfolding backtrack.simps
+      apply (simp add: is_decision_lit_def)
+      sorry
+  next
+    case (Some a)
+    then show ?thesis sorry
+  qed
+  oops
+
+lemma ball_trail_defined_lit_if:
+  assumes
+    no_conflict: "state_conflict S = None" and
+    (* no_propagate: "\<nexists>S'. propagate N S S'" and *)
+    no_decide: "\<nexists>S'. decide N S S'" (* and
+    no_new_conflict: "\<nexists>S'. conflict N S S'" *)
+  shows "\<forall>C \<in> N. \<forall>L \<in># C. \<forall>\<gamma>. is_ground_lit (L \<cdot>l \<gamma>) \<longrightarrow> trail_defined_lit (state_trail S) (L \<cdot>l \<gamma>)"
+proof (intro ballI allI impI)
+  fix C L \<gamma>
+  assume "C \<in> N" "L \<in># C" "is_ground_lit (L \<cdot>l \<gamma>)"
+
+  from no_conflict obtain \<Gamma> U where S_def: "S = (\<Gamma>, U, None)"
+    by (metis prod_cases3 state_conflict_simp)
+
+  show "trail_defined_lit (state_trail S) (L \<cdot>l \<gamma>)"
+    using no_decide
+  proof (rule contrapos_np)
+    assume assm: "\<not> trail_defined_lit (state_trail S) (L \<cdot>l \<gamma>)"
+    show "\<exists>S'. decide N S S'"
+      using decideI[OF \<open>is_ground_lit (L \<cdot>l \<gamma>)\<close> assm]
+      unfolding S_def state_trail_simp
+      by fastforce
+  qed
+qed
+
+lemma trail_defined_lit_iff: "trail_defined_lit \<Gamma> L \<longleftrightarrow> atm_of L \<in> atm_of ` fst ` set \<Gamma>"
+  by (simp add: atm_of_in_atm_of_set_iff_in_set_or_uminus_in_set trail_defined_lit_def)
+
+lemma "trail_interp \<Gamma> \<subseteq> atm_of ` fst ` set \<Gamma>"
+  by (smt (verit, best) UN_iff image_iff insert_iff literal.case_eq_if singletonD subsetI trail_interp_def)
+
+lemma set_filter_insert_conv:
+  "{x \<in> insert y S. P x} = (if P y then insert y else id) {x \<in> S. P x}"
+  by auto
+
+lemma trail_interp_conv: "trail_interp \<Gamma> = atm_of ` {L \<in> fst ` set \<Gamma>. is_pos L}"
+proof (induction \<Gamma>)
+  case Nil
+  show ?case by (simp add: trail_interp_def)
+next
+  case (Cons Ln \<Gamma>)
+  then show ?case
+    unfolding list.set image_insert set_filter_insert_conv trail_interp_Cons'
+    by (simp add: literal.case_eq_if)
+qed
+
+lemma not_in_trail_interp_if_not_in_trail: "t \<notin> atm_of ` fst ` set \<Gamma> \<Longrightarrow> t \<notin> trail_interp \<Gamma>"
+  by (metis (no_types, lifting) atm_of_in_atm_of_set_iff_in_set_or_uminus_in_set
+      literal.sel(2) mem_Collect_eq trail_interp_conv)
+
+lemma trail_interp_lit_if_sound_and_trail_true:
+  shows "sound_trail N U \<Gamma> \<Longrightarrow> trail_true_lit \<Gamma> L \<Longrightarrow> trail_interp \<Gamma> \<TTurnstile>l L"
+proof (induction \<Gamma> rule: sound_trail.induct)
+  case Nil
+  thus ?case
+    by (simp add: trail_true_lit_def)
+next
+  case (Cons \<Gamma> K u)
+  show ?case
+  proof (cases "L = K \<or> L = - K")
+    case True
+    then show ?thesis 
+    proof (elim disjE)
+      assume "L = K"
+      thus ?thesis
+      proof (cases L; cases K)
+        fix t\<^sub>L t\<^sub>K
+        from \<open>L = K\<close> show "L = Pos t\<^sub>L \<Longrightarrow> K = Pos t\<^sub>K \<Longrightarrow> ?thesis"
+          by (simp add: trail_interp_def)
+      next
+        fix t\<^sub>L t\<^sub>K
+        from \<open>L = K\<close> show "L = Neg t\<^sub>L \<Longrightarrow> K = Neg t\<^sub>K \<Longrightarrow> ?thesis"
+          using Cons.hyps
+          by (simp add: trail_defined_lit_iff trail_interp_Cons'
+              not_in_trail_interp_if_not_in_trail)
+      qed simp_all
+    next
+      assume "L = - K"
+      then show ?thesis
+      proof (cases L; cases K)
+        fix t\<^sub>L t\<^sub>K
+        from \<open>L = - K\<close> show "L = Pos t\<^sub>L \<Longrightarrow> K = Neg t\<^sub>K \<Longrightarrow> ?thesis"
+          unfolding trail_interp_Cons'
+          using Cons.hyps(1) Cons.prems
+          by (metis (no_types, lifting) image_insert insertE list.simps(15) literal.distinct(1)
+              prod.sel(1) trail_defined_lit_def trail_true_lit_def)
+      next
+        fix t\<^sub>L t\<^sub>K
+        from \<open>L = - K\<close> show "L = Neg t\<^sub>L \<Longrightarrow> K = Pos t\<^sub>K \<Longrightarrow> ?thesis"
+          unfolding trail_interp_Cons'
+          using Cons.hyps(1) Cons.prems
+          by (metis (no_types, lifting) image_insert insertE list.simps(15) literal.distinct(1)
+              prod.sel(1) trail_defined_lit_def trail_true_lit_def)
+      qed simp_all
+    qed
+  next
+    case False
+    with Cons.prems have "trail_true_lit \<Gamma> L"
+      by (simp add: trail_true_lit_def)
+    with Cons.IH have "trail_interp \<Gamma> \<TTurnstile>l L"
+      by simp
+    with False show ?thesis
+      by (cases L; cases K) (simp_all add: trail_interp_def del: true_lit_iff)
+  qed
+qed
+
+lemma trail_interp_cls_if_sound_and_trail_true:
+  assumes "sound_trail N U \<Gamma>" and "trail_true_cls \<Gamma> C"
+  shows "trail_interp \<Gamma> \<TTurnstile> C"
+proof -
+  from \<open>trail_true_cls \<Gamma> C\<close> obtain L where "L \<in># C" and "trail_true_lit \<Gamma> L"
+    by (auto simp: trail_true_cls_def)
+  show ?thesis
+    unfolding true_cls_def
+  proof (rule bexI[OF _ \<open>L \<in># C\<close>])
+    show "trail_interp \<Gamma> \<TTurnstile>l L"
+      by (rule trail_interp_lit_if_sound_and_trail_true[OF \<open>sound_trail N U \<Gamma>\<close> \<open>trail_true_lit \<Gamma> L\<close>])
+  qed
+qed
+
+lemma set_removeAll_mset: "set_mset (removeAll_mset x M) = set_mset M - {x}"
+  by simp
+
+lemma trail_true_lit_Cons_iff: "trail_true_lit ((L, u) # \<Gamma>) K \<longleftrightarrow> L = K \<or> trail_true_lit \<Gamma> K"
+  by (auto simp: trail_true_lit_def)
+
+lemma trail_true_cls_Cons_iff: "trail_true_cls ((L, u) # \<Gamma>) C \<longleftrightarrow> L \<in># C \<or> trail_true_cls \<Gamma> C"
+  by (auto simp: trail_true_cls_def trail_true_lit_Cons_iff)
+
+lemma trail_true_cls_iff_trail_interp_entails:
+  assumes "sound_trail N U \<Gamma>" "\<forall>L \<in># C. trail_defined_lit \<Gamma> L"
+  shows "trail_true_cls \<Gamma> C \<longleftrightarrow> trail_interp \<Gamma> \<TTurnstile> C"
+proof (rule iffI)
+  assume "trail_true_cls \<Gamma> C"
+  thus "trail_interp \<Gamma> \<TTurnstile> C"
+    using assms(1) trail_interp_cls_if_sound_and_trail_true by blast
+next
+  assume "trail_interp \<Gamma> \<TTurnstile> C"
+  then obtain L where "L \<in># C" and "trail_interp \<Gamma> \<TTurnstile>l L"
+    by (auto simp: true_cls_def)
+  show "trail_true_cls \<Gamma> C"
+  proof (cases L)
+    case (Pos t)
+    hence "t \<in> trail_interp \<Gamma>"
+      using \<open>trail_interp \<Gamma> \<TTurnstile>l L\<close> by simp
+    then show ?thesis
+      unfolding trail_true_cls_def
+      using \<open>L \<in># C\<close> Pos
+      by (metis assms(1) assms(2) trail_defined_lit_def trail_interp_lit_if_sound_and_trail_true
+          trail_true_lit_def true_lit_simps(2) uminus_Pos)
+  next
+    case (Neg t)
+    then show ?thesis
+      by (metis \<open>L \<in># C\<close> \<open>trail_interp \<Gamma> \<TTurnstile>l L\<close> assms(1) assms(2) trail_defined_lit_def
+          trail_interp_lit_if_sound_and_trail_true trail_true_cls_def trail_true_lit_def
+          true_lit_simps(1) true_lit_simps(2) uminus_Neg)
+  qed
+qed
+
+lemma trail_interp_clss_if_sound_and_trail_true:
+  assumes "sound_trail N U \<Gamma>" and "trail_true_clss \<Gamma> CC"
+  shows "trail_interp \<Gamma> \<TTurnstile>s CC"
+  using \<open>trail_true_clss \<Gamma> CC\<close> trail_interp_cls_if_sound_and_trail_true[OF \<open>sound_trail N U \<Gamma>\<close>]
+  by (simp add: trail_true_clss_def true_clss_def)
+
+lemma
+  assumes
+    fin_N: "finite N" and disj_N: "disjoint_vars_set N" and
+    regular_run: "(regular_scl N)\<^sup>*\<^sup>* initial_state S" and
+    no_more_regular_step: "\<nexists>S'. regular_scl N S S'"
+  shows "\<not> satisfiable (grounding_of_clss N) \<and> (\<exists>\<gamma>. state_conflict S = Some ({#}, \<gamma>)) \<or>
+  (\<exists>\<gamma>. trail_true_clss (state_trail S) (N \<cdot>cs \<gamma>))"
+proof -
+  obtain \<Gamma> U u where S_def: "S = (\<Gamma>, U, u)"
+    using prod_cases3 by blast
+
+  have sound_S: "sound_state N S"
+    using regular_run_sound_state[OF regular_run] sound_initial_state[OF fin_N disj_N] by blast
+
+  from no_more_regular_step have no_new_conflict: "\<nexists>S'. conflict N S S'"
+    using regular_scl_def by blast
+
+  from no_more_regular_step have no_propagate: "\<nexists>S'. propagate N S S'"
+    by (meson decide_well_defined(1) local.scl_def reasonable_scl_def regular_scl_def)
+
+  from no_more_regular_step have
+    no_reasonable_decide: "(\<nexists>S'. decide N S S') \<or> (\<exists>S' S''. decide N S S' \<and> conflict N S' S'')"
+    using local.scl_def reasonable_scl_def regular_scl_def by blast
+
+  show ?thesis
+  proof (cases u)
+    case None
+    hence "state_conflict S = None"
+      by (simp add: S_def)
+    
+    have ball_N_not_empty: "\<forall>C \<in> N. C \<noteq> {#}" sorry
+
+    have "satisfiable (grounding_of_clss N)"
+      using trail_interp_clss_if_sound_and_trail_true[OF ]
+      (* using sound_S[unfolded S_def None] *)
+      apply (rule exI[where x = "trail_interp \<Gamma>"])
+      unfolding true_clss_def true_cls_def grounding_of_clss_def grounding_of_cls_def
+      unfolding imp_ex ball_UN ball_simps
+            
+      unfolding sound_state_def
+      sorry
+    moreover have "\<exists>\<gamma>. trail_true_clss \<Gamma> (N \<cdot>cs \<gamma>)"
+      using no_more_regular_step
+      unfolding S_def[unfolded None]
+      unfolding regular_scl_def
+      sorry
+    ultimately show ?thesis
+      unfolding S_def[unfolded None] state_trail_def state_conflict_def prod.sel
+      by simp
+  next
+    case (Some Cl)
+    then obtain C \<gamma> where u_def: "u = Some (C, \<gamma>)" by force
+    show ?thesis
+    proof (cases "C = {#}")
+      case True
+      hence "\<not> satisfiable (grounding_of_clss N) \<and> (\<exists>\<gamma>. state_conflict S = Some ({#}, \<gamma>))"
+        using S_def u_def not_satisfiable_if_sound_state_conflict_bottom[OF sound_S] by simp
+      thus ?thesis by simp
+    next
+      case False
+      then obtain L C' where C_def: "C = C' + {#L#}"
+        by (metis add_mset_add_single multi_nonempty_split)
+
+      from no_more_regular_step have "\<nexists>S'. (reasonable_scl N)\<^sup>+\<^sup>+ (\<Gamma>, U, Some (C' + {#L#}, \<gamma>)) S'"
+        unfolding S_def u_def C_def
+        unfolding regular_scl_def
+        sorry
+
+      then have False
+        unfolding reasonable_scl_def
+        sorry
+
+      then show ?thesis by simp
+    qed
+  qed
+  oops
 
 section \<open>Clause Redundancy\<close>
+
+term is_ground_clss
 
 definition ground_redundant where
   "ground_redundant lt N C \<longleftrightarrow> is_ground_clss N \<and> is_ground_cls C \<and> {D \<in> N. lt\<^sup>=\<^sup>= D C} \<TTurnstile>e {C}"
@@ -2496,6 +3626,59 @@ lemma total_on_trail_less_ex:
   by (smt (verit, ccfv_threshold) Restricted_Predicates.total_on_def defined_conv
       uminus_uminus_id)
 
+
+subsection \<open>Properties\<close>
+
+lemma trail_defined_if_trail_less_ex:
+  "trail_less_ex lt (map fst \<Gamma>) L K \<Longrightarrow> trail_defined_lit \<Gamma> K \<Longrightarrow> trail_defined_lit \<Gamma> L"
+  by (metis (no_types, opaque_lifting) list.set_map trail_defined_lit_def trail_less_ex_def)
+
+lemma total_on_unionD:
+  assumes "Restricted_Predicates.total_on R (S1 \<union> S2)"
+  shows
+    total_on_unionD1: "Restricted_Predicates.total_on R S1" and
+    total_on_unionD2: "Restricted_Predicates.total_on R S2"
+  by (metis Un_iff assms total_on_conv)+
+
+lemma trail_defined_cls_if_lt_defined:
+  assumes sound_\<Gamma>: "sound_trail N U \<Gamma>" and
+    transp_lt: "transp lt" and
+    total_on_lt: "Restricted_Predicates.total_on lt (set_mset C \<union> set_mset D)" and
+    C_lt_D: "multp (trail_less_ex lt (map fst \<Gamma>)) C D" and
+    tr_def_D: "trail_defined_cls \<Gamma> D"
+  shows "trail_defined_cls \<Gamma> C"
+proof -
+  have transp_on: "transp_on (trail_less_ex lt (map fst \<Gamma>)) S" for S
+    using transp_trail_less_ex_if_sound[OF sound_\<Gamma> transp_lt]
+    by (metis transpD transp_onI)
+
+  have tot_on_C_D:
+    "Restricted_Predicates.total_on (trail_less_ex lt (map fst \<Gamma>)) (set_mset C \<union> set_mset D)"
+    using total_on_trail_less_ex[OF Clausal_Logic.uminus_of_uminus_id total_on_lt]
+    by assumption
+
+  show ?thesis
+    using total_on_unionD[
+        OF tot_on_C_D,
+        THEN multiset_is_empty_or_bex_greatest_element_if_trans_and_total[OF transp_on]]
+  proof (elim disjE)
+    assume
+      "\<exists>x\<in>#C. \<forall>y\<in>#C. x \<noteq> y \<longrightarrow> trail_less_ex lt (map fst \<Gamma>) y x"
+      "D = {#}"
+    thus "trail_defined_cls \<Gamma> C"
+      using C_lt_D multp_implies_one_step sound_\<Gamma> transp_lt transp_trail_less_ex_if_sound
+      by blast
+  next
+    assume
+      "\<exists>x\<in>#C. \<forall>y\<in>#C. x \<noteq> y \<longrightarrow> trail_less_ex lt (map fst \<Gamma>) y x"
+      "\<exists>x\<in>#D. \<forall>y\<in>#D. x \<noteq> y \<longrightarrow> trail_less_ex lt (map fst \<Gamma>) y x"
+    show "trail_defined_cls \<Gamma> C"
+      using tr_def_D trail_defined_if_trail_less_ex
+      by (smt (verit, ccfv_threshold) C_lt_D multp_implies_one_step sound_\<Gamma> trail_defined_cls_def
+          transp_lt transp_trail_less_ex_if_sound union_iff)
+  qed (simp_all add: trail_defined_cls_def)
+qed
+
 lemma wfP_trail_less_ex:
   fixes Ls :: "('a :: uminus) list"
   assumes
@@ -2523,6 +3706,953 @@ proof (intro allI impI)
       by (metis (no_types, lifting) IntD1 IntD2 UnE defined_conv trail_less_ex_def uminus_uminus_id)
   qed
 qed
+
+section \<open>Learned Clauses in Regular Runs\<close>
+
+term multp
+term "multp (trail_less_ex lt (map fst \<Gamma>))"
+term "redundant (multp (trail_less_ex lt (map fst \<Gamma>)))"
+
+term "regular_scl N initial_state"
+
+thm regular_scl_def
+thm ground_redundant_def redundant_def
+
+lemma
+  assumes "sound_state N S" and "conflict N S S'"
+  shows "redundant (multp (trail_less_ex lt (map fst (state_trail S))))
+    (N \<union> state_learned S) (fst (the (state_conflict S')))"
+proof -
+  from \<open>conflict N S S'\<close> obtain \<Gamma> U C \<gamma> where
+    S_def: "S = (\<Gamma>, U, None)" and S'_def: "S' = (\<Gamma>, U, Some (C, \<gamma>))"
+    by (smt (verit) conflict.simps)
+
+  from \<open>conflict N S S'\<close> obtain C' where
+    "C' \<in> N \<union> U" and
+    "C = rename_clause (N \<union> U \<union> clss_of_trail \<Gamma>) C'" and
+    "subst_domain \<gamma> \<subseteq> vars_cls C" and
+    "is_ground_cls (C \<cdot> \<gamma>)" and
+    "trail_false_cls \<Gamma> (C \<cdot> \<gamma>)"
+    by (auto simp: S_def S'_def elim!: conflict.cases)
+
+  then show ?thesis
+    using assms(1)
+    apply (simp add: S_def S'_def sound_state_def redundant_def ground_redundant_def
+        grounding_of_cls_rename_clause is_ground_cls_if_in_grounding_of_cls)
+    by (smt (verit, best) UN_I \<open>C' \<in> N \<union> U\<close> grounding_of_clss_def mem_Collect_eq true_clss_def)
+qed
+
+lemma assumes "asymp lt" and "transp lt" and "sound_state N S" and "resolve N S S'"
+  shows "\<not> redundant (multp (trail_less_ex lt (map fst (state_trail S))))
+    (N \<union> state_learned S) (fst (the (state_conflict S')))"
+proof (rule notI)
+  from \<open>resolve N S S'\<close> \<open>sound_state N S\<close> have "sound_state N S'"
+    by (rule resolve_sound_state)
+
+  from \<open>resolve N S S'\<close> obtain \<Gamma> \<Gamma>' L C \<delta> D \<sigma> \<rho> U L' \<mu> where
+    S_def: "S = (\<Gamma>, U, Some (D + {#L'#}, \<sigma>))" and
+    S'_def: "S' = (\<Gamma>, U, Some ((D + C) \<cdot> \<mu> \<cdot> \<rho>,
+      restrict_subst (vars_cls ((D + C) \<cdot> \<mu> \<cdot> \<rho>)) (inv_renaming' \<rho> \<odot> \<sigma> \<odot> \<delta>)))" and
+    "\<Gamma> = trail_propagate \<Gamma>' L C \<delta>" and
+    "trail_level_cls \<Gamma> (D \<cdot> \<sigma>) = trail_level \<Gamma>" and
+    "\<rho> = renaming_wrt (N \<union> U \<union> clss_of_trail \<Gamma> \<union> {D + {#L'#}})" and
+    "L \<cdot>l \<delta> = - (L' \<cdot>l \<sigma>)" and
+    "Unification.mgu (atm_of L) (atm_of L') = Some \<mu>"
+    by (cases N S S' rule: resolve.cases) simp_all
+
+  define \<gamma> where "\<gamma> = restrict_subst (vars_cls ((D + C) \<cdot> \<mu> \<cdot> \<rho>)) (inv_renaming' \<rho> \<odot> \<sigma> \<odot> \<delta>)"
+  define lt' where "lt' = multp (trail_less_ex lt (map fst \<Gamma>))"
+
+  from \<open>sound_state N S'\<close> have "sound_trail N U \<Gamma>" and "trail_false_cls \<Gamma> ((D + C) \<cdot> \<mu> \<cdot> \<rho> \<cdot> \<gamma>)"
+    by (simp_all add: sound_state_def S'_def \<gamma>_def)
+
+  assume "redundant (multp (trail_less_ex lt (map fst (state_trail S))))
+    (N \<union> state_learned S) (fst (the (state_conflict S')))"
+  hence "redundant lt' (N \<union> U) ((D + C) \<cdot> \<mu> \<cdot> \<rho>)"
+    by (simp add: S_def S'_def lt'_def)
+  moreover from \<open>sound_state N S'\<close> have "is_ground_cls ((D + C) \<cdot> \<mu> \<cdot> \<rho> \<cdot> \<gamma>)"
+    unfolding S'_def sound_state_def \<gamma>_def by simp
+  ultimately have "ground_redundant lt' (grounding_of_clss (N \<union> U)) ((D + C) \<cdot> \<mu> \<cdot> \<rho> \<cdot> \<gamma>)"
+    unfolding redundant_def
+    by (metis grounding_of_cls_ground insert_subset subst_cls_eq_grounding_of_cls_subset_eq)
+  hence gr_entails_gr:
+    "{E \<in> grounding_of_clss (N \<union> U). lt'\<^sup>=\<^sup>= E ((D + C) \<cdot> \<mu> \<cdot> \<rho> \<cdot> \<gamma>)} \<TTurnstile>e {(D + C) \<cdot> \<mu> \<cdot> \<rho> \<cdot> \<gamma>}"
+    by (simp add: ground_redundant_def)
+
+  have "E \<in> {E \<in> grounding_of_clss (N \<union> U). lt'\<^sup>=\<^sup>= E ((D + C) \<cdot> \<mu> \<cdot> \<rho> \<cdot> \<gamma>)} \<Longrightarrow>
+    trail_defined_lit \<Gamma> L" if "L \<in># E" for E L
+    unfolding mem_Collect_eq Lattices.sup_apply sup_bool_def
+  proof (elim conjE disjE)
+    note trans = transp_trail_less_ex_if_sound[OF \<open>sound_trail N U \<Gamma>\<close> \<open>transp lt\<close>]
+
+    assume "E \<in> grounding_of_clss (N \<union> U)" and "lt' E ((D + C) \<cdot> \<mu> \<cdot> \<rho> \<cdot> \<gamma>)"
+    then show ?thesis
+      using multiset_is_empty_or_bex_greatest_element_if_trans_and_total[OF ]
+      using total_on_trail_less_ex
+      sorry
+
+    (* hence "multp\<^sub>H\<^sub>O (trail_less_ex lt (map fst \<Gamma>)) E ((D + C) \<cdot> \<mu> \<cdot> \<rho> \<cdot> \<gamma>)"
+      unfolding lt'_def
+      using transp_trail_less_ex_if_sound[OF \<open>sound_trail N U \<Gamma>\<close> \<open>transp lt\<close>]
+      using asymp_trail_less_ex_if_sound[OF \<open>sound_trail N U \<Gamma>\<close> \<open>asymp lt\<close>]
+      by (simp add: multp_eq_multp\<^sub>H\<^sub>O)
+    then show ?thesis
+      unfolding multp\<^sub>H\<^sub>O_def
+      using \<open>trail_false_cls \<Gamma> ((D + C) \<cdot> \<mu> \<cdot> \<rho> \<cdot> \<gamma>)\<close>[unfolded trail_false_cls_def]
+      using \<open>L \<in># E\<close>
+      sorry *)
+  next
+    assume "E \<in> grounding_of_clss (N \<union> U)" and "E = (D + C) \<cdot> \<mu> \<cdot> \<rho> \<cdot> \<gamma>"
+    with that and \<open>trail_false_cls \<Gamma> ((D + C) \<cdot> \<mu> \<cdot> \<rho> \<cdot> \<gamma>)\<close> show ?thesis
+      using trail_defined_lit_iff_true_or_false trail_false_cls_def by blast
+  qed
+
+  obtain E where
+    "E \<in> {E \<in> grounding_of_clss (N \<union> U). lt'\<^sup>=\<^sup>= E ((D + C) \<cdot> \<mu> \<cdot> \<rho> \<cdot> \<gamma>)} \<and> trail_false_cls \<Gamma> E"
+    sorry
+
+  then show False
+    using \<open>trail_false_cls \<Gamma> ((D + C) \<cdot> \<mu> \<cdot> \<rho> \<cdot> \<gamma>)\<close>
+    using gr_entails_gr[rule_format, of "trail_interp \<Gamma>"] contrapos_pp
+    apply (simp add: \<open>is_ground_cls ((D + C) \<cdot> \<mu> \<cdot> \<rho> \<cdot> \<gamma>)\<close>)
+    oops
+
+lemma regular_run_if_skip_factorize_resolve_run:
+  assumes "(\<lambda>S S'. skip N S S' \<or> factorize N S S' \<or> resolve N S S')\<^sup>*\<^sup>* S S'"
+  shows "(regular_scl N)\<^sup>*\<^sup>* S S'"
+  using assms
+  by (smt (verit, ccfv_SIG) decide_well_defined(4) decide_well_defined(5) local.scl_def
+      mono_rtranclp reasonable_scl_def regular_scl_def skip_well_defined(2))
+
+lemma trail_false_conflict_after_skip:
+  assumes
+    conflict_S: "state_conflict S = Some (C, \<gamma>)" and
+    false_C_\<gamma>: "trail_false_cls (state_trail S) (C \<cdot> \<gamma>)" and
+    "skip N S S'"
+  shows "state_conflict S' = Some (C, \<gamma>) \<and> trail_false_cls (state_trail S) (C \<cdot> \<gamma>)"
+  using \<open>skip N S S'\<close>
+proof (cases N S S' rule: skip.cases)
+  case (skipI L \<delta> D \<sigma> \<Gamma> C U)
+  then show ?thesis
+    using conflict_S false_C_\<gamma>
+    by (auto elim!: trail_false_cls_ConsD simp add: sound_state_def trail_propagate_def)
+qed
+
+lemma strict_suffix_trail_if_skip: "skip N S S' \<Longrightarrow> strict_suffix (state_trail S') (state_trail S)"
+  by (auto simp: skip.simps strict_suffix_def suffix_def trail_propagate_def)
+
+lemma eq_trail_if_factorize: "factorize N S S' \<Longrightarrow> state_trail S' = state_trail S"
+  by (auto simp: factorize.simps)
+
+lemma eq_trail_if_resolve: "resolve N S S' \<Longrightarrow> state_trail S' = state_trail S"
+  by (auto simp: resolve.simps)
+
+lemma not_trail_true_and_false_lit:
+  "sound_trail N U \<Gamma> \<Longrightarrow> \<not> (trail_true_lit \<Gamma> L \<and> trail_false_lit \<Gamma> L)"
+  apply (simp add: trail_true_lit_def trail_false_lit_def)
+  by (metis (no_types, lifting) in_set_conv_nth list.set_map pairwise_distinct_if_sound_trail
+      uminus_not_id')
+
+lemma not_trail_true_and_false_cls: "sound_trail N U \<Gamma> \<Longrightarrow> \<not> (trail_true_cls \<Gamma> C \<and> trail_false_cls \<Gamma> C)"
+  using not_trail_true_and_false_lit
+  by (metis trail_false_cls_def trail_true_cls_def)
+
+lemma conflict_if_mempty_in_clause_set:
+  assumes "{#} \<in> N" and "state_conflict S1 = None"
+  shows "\<exists>S2. conflict N S1 S2 \<and> state_conflict S2 = Some ({#}, Var)"
+proof -
+  from \<open>state_conflict S1 = None\<close> obtain \<Gamma> U where S1_def: "S1 = (\<Gamma>, U, None)"
+    by (metis prod.collapse state_conflict_def)
+
+  show ?thesis
+  proof (intro exI conjI)
+    from \<open>{#} \<in> N\<close> show "conflict N S1 (\<Gamma>, U, Some ({#}, Var))"
+      by (auto simp: S1_def conflict.simps)
+  next
+    show "state_conflict (\<Gamma>, U, Some ({#}, Var)) = Some ({#}, Var)"
+      by simp
+  qed
+qed
+
+definition trail_no_conflict where
+  "trail_no_conflict N \<Gamma> \<longleftrightarrow> (\<nexists>C \<gamma>. C \<in> N \<and> trail_false_cls \<Gamma> (C \<cdot> \<gamma>))"
+
+lemma trail_no_conflict_initial_state:
+  assumes "{#} \<notin> N"
+  shows "trail_no_conflict (N \<union> state_learned initial_state) (state_trail initial_state)"
+  unfolding trail_no_conflict_def
+  apply simp
+  by (metis assms not_trail_false_Nil(2) subst_cls_empty_iff)
+
+definition trail_almost_no_conflict where
+  "trail_almost_no_conflict N \<Gamma> \<longleftrightarrow> trail_no_conflict N (trail_backtrack \<Gamma> (trail_level \<Gamma>))"
+
+lemma trail_false_cls_if_suffix_and_false:
+  "suffix \<Gamma> \<Gamma>' \<Longrightarrow> trail_false_cls \<Gamma> C \<Longrightarrow> trail_false_cls \<Gamma>' C"
+  unfolding trail_false_cls_def suffix_def
+  by (elim exE) (auto simp add: trail_false_lit_def)
+
+lemma trail_no_conflict_suffixI:
+  "suffix \<Gamma> \<Gamma>' \<Longrightarrow> trail_no_conflict N \<Gamma>' \<Longrightarrow> trail_no_conflict N \<Gamma>"
+  unfolding trail_no_conflict_def
+  apply (erule contrapos_nn)
+  apply (elim exE)
+  using trail_false_cls_if_suffix_and_false by blast
+
+lemma trail_almost_no_conflict_if_trail_no_conflict:
+  "trail_no_conflict N \<Gamma> \<Longrightarrow> trail_almost_no_conflict N \<Gamma>"
+  unfolding trail_almost_no_conflict_def trail_no_conflict_def
+  using trail_backtrack_suffix[of \<Gamma>, THEN trail_false_cls_if_suffix_and_false]
+  by (elim contrapos_nn) blast
+
+lemma
+  assumes suff: "suffix \<Gamma>' \<Gamma>" and "trail_almost_no_conflict N \<Gamma>"
+  shows "trail_almost_no_conflict N \<Gamma>'"
+proof -
+  from suff have "suffix (trail_backtrack \<Gamma>' (trail_level \<Gamma>')) \<Gamma>"
+    using trail_backtrack_suffix[of \<Gamma>']
+    using suffix_order.order_trans by blast
+  then show ?thesis
+    unfolding trail_almost_no_conflict_def
+    using trail_no_conflict_suffixI trail_almost_no_conflict_if_trail_no_conflict
+    oops
+
+definition regular_state where
+  "regular_state N S \<longleftrightarrow> sound_state N S \<and> (\<exists>\<Gamma> U u. S = (\<Gamma>, U, u) \<and>
+      trail_almost_no_conflict (N \<union> U \<union> (case u of None \<Rightarrow> {} | Some (C, \<gamma>) \<Rightarrow> {C})) \<Gamma>)"
+
+lemma conflict_preserves_trail_almost_no_conflict:
+  assumes "conflict N S1 S2" and "trail_almost_no_conflict (N \<union> state_learned S1) (state_trail S1)"
+  shows "trail_almost_no_conflict (N \<union> state_learned S2) (state_trail S2)"
+  using assms by (auto simp: conflict.simps)
+
+lemma conflict_regular_state:
+  assumes step: "conflict N S1 S2" and "regular_state N S1"
+  shows "regular_state N S2"
+  using step
+proof (cases N S1 S2 rule: conflict.cases)
+  case (conflictI D U D' \<Gamma> \<sigma>)
+  with \<open>regular_state N S1\<close> have
+    sound_S1: "sound_state N S1" and
+    tr_almost_no_conf: "trail_almost_no_conflict (N \<union> U) \<Gamma>"
+    by (simp_all add: regular_state_def)
+
+  show ?thesis
+    unfolding regular_state_def
+  proof (intro conjI exI)
+    show "sound_state N S2"
+      by (rule conflict_sound_state[OF step sound_S1])
+  next
+    show "S2 = (\<Gamma>, U, Some (D', \<sigma>))"
+      using conflictI by simp
+  next
+    show "trail_almost_no_conflict
+      (N \<union> U \<union> (case Some (D', \<sigma>) of None \<Rightarrow> {} | Some (C, \<gamma>) \<Rightarrow> {C})) \<Gamma>"
+      apply simp
+      using tr_almost_no_conf
+      unfolding trail_almost_no_conflict_def
+      unfolding trail_no_conflict_def
+      using conflictI
+      by (metis insertE rename_clause_def subst_cls_comp_subst)
+  qed
+qed
+
+lemma propagate_preserves_trail_backtrack_level: "propagate N S1 S2 \<Longrightarrow>
+  (let \<Gamma> = state_trail S1 in trail_backtrack \<Gamma> (trail_level \<Gamma>)) =
+  (let \<Gamma> = state_trail S2 in trail_backtrack \<Gamma> (trail_level \<Gamma>))"
+  by (auto simp add: propagate.simps)
+
+lemma propagate_preserves_trail_almost_no_conflict:
+  assumes "propagate N S1 S2" and "trail_almost_no_conflict (N \<union> state_learned S1) (state_trail S1)"
+  shows "trail_almost_no_conflict (N \<union> state_learned S2) (state_trail S2)"
+  using assms by (auto simp add: propagate.simps trail_almost_no_conflict_def)
+
+lemma propagate_regular_state:
+  assumes step: "propagate N S1 S2" and "regular_state N S1"
+  shows "regular_state N S2"
+  using step
+proof (cases N S1 S2 rule: propagate.cases)
+  case (propagateI C U C'' L \<Gamma> \<gamma>)
+  with \<open>regular_state N S1\<close> have
+    sound_S1: "sound_state N S1" and
+    tr_almost_no_conf: "trail_almost_no_conflict (N \<union> U) \<Gamma>"
+    by (simp_all add: regular_state_def)
+  show ?thesis
+    unfolding regular_state_def
+  proof (intro conjI exI)
+    show "sound_state N S2"
+      by (rule propagate_sound_state[OF step sound_S1])
+  next
+    show "S2 = (trail_propagate \<Gamma> L C'' \<gamma>, U, None)"
+      using propagateI by simp
+  next
+    show "trail_almost_no_conflict
+      (N \<union> U \<union> (case None of None \<Rightarrow> {} | Some (C, \<gamma>) \<Rightarrow> {C})) (trail_propagate \<Gamma> L C'' \<gamma>)"
+      apply simp
+      using tr_almost_no_conf
+      by (simp add: trail_almost_no_conflict_def)
+  qed
+qed
+
+lemma skip_regular_state:
+  assumes step: "skip N S1 S2" and "regular_state N S1"
+  shows "regular_state N S2"
+  using step
+proof (cases N S1 S2 rule: skip.cases)
+  case (skipI L \<delta> D \<sigma> \<Gamma> C U)
+  with \<open>regular_state N S1\<close> have
+    sound_S1: "sound_state N S1" and
+    tr_almost_no_conf: "trail_almost_no_conflict (N \<union> U \<union> {D}) (trail_propagate \<Gamma> L C \<delta>)"
+    by (simp_all add: regular_state_def)
+  show ?thesis
+    unfolding regular_state_def
+  proof (intro conjI exI)
+    show "sound_state N S2"
+      by (rule skip_sound_state[OF step sound_S1])
+  next
+    show "S2 = (\<Gamma>, U, Some (D, \<sigma>))"
+      using skipI by simp
+  next
+    show "trail_almost_no_conflict
+      (N \<union> U \<union> (case Some (D, \<sigma>) of None \<Rightarrow> {} | Some (C, \<gamma>) \<Rightarrow> {C})) \<Gamma>"
+      apply simp
+      using tr_almost_no_conf
+      by (simp add: trail_almost_no_conflict_def)
+  qed
+qed
+
+lemma factorize_regular_state:
+  assumes step: "factorize N S1 S2" and "regular_state N S1"
+  shows "regular_state N S2"
+  using step
+proof (cases N S1 S2 rule: factorize.cases)
+  case (factorizeI L \<sigma> L' \<mu> \<sigma>' D \<Gamma> U)
+  with \<open>regular_state N S1\<close> have
+    sound_S1: "sound_state N S1" and
+    tr_almost_no_conf: "trail_almost_no_conflict (N \<union> U \<union> {D + {#L, L'#}}) \<Gamma>"
+    by (simp_all add: regular_state_def)
+  show ?thesis
+    unfolding regular_state_def
+  proof (intro conjI exI)
+    show "sound_state N S2"
+      by (rule factorize_sound_state[OF step sound_S1])
+  next
+    show "S2 = (\<Gamma>, U, Some ((D + {#L#}) \<cdot> \<mu>, \<sigma>'))"
+      using factorizeI by simp
+  next
+    show "trail_almost_no_conflict
+      (N \<union> U \<union> (case Some ((D + {#L#}) \<cdot> \<mu>, \<sigma>') of None \<Rightarrow> {} | Some (C, \<gamma>) \<Rightarrow> {C})) \<Gamma>"
+      apply simp
+      using tr_almost_no_conf
+      apply (simp add: trail_almost_no_conflict_def)
+      unfolding trail_no_conflict_def
+      apply (erule contrapos_nn)
+      apply (elim exE conjE)
+        unfolding insert_iff
+        apply (erule disjE)
+        subgoal for C \<gamma>
+          apply (rule exI[of _ "add_mset L (add_mset L' D)"])
+          apply (rule exI[of _ "\<mu> \<odot> \<gamma>"])
+          apply simp
+          by (metis (mono_tags, lifting) atm_of_subst_lit insert_iff literal.expand factorizeI(3)
+              factorizeI(4) set_mset_add_mset_insert subst_lit_is_neg subst_term_eq_if_mgu
+              trail_false_cls_def)
+        subgoal for C \<gamma>
+          by blast
+        done
+  qed
+qed
+
+lemma resolve_regular_state:
+  fixes N :: "('f, 'v) term clause set"
+  assumes step: "resolve N S1 S2" and "regular_state N S1"
+  shows "regular_state N S2"
+  using step
+proof (cases N S1 S2 rule: resolve.cases)
+  case (resolveI \<Gamma> \<Gamma>' L C \<delta> D \<sigma> \<rho> U L' \<mu>)
+  with \<open>regular_state N S1\<close> have
+    sound_S1: "sound_state N S1" and
+    tr_almost_no_conf: "trail_almost_no_conflict (N \<union> U \<union> {D + {#L'#}}) \<Gamma>"
+    by (simp_all add: regular_state_def)
+
+  let ?\<gamma> = "restrict_subst (vars_cls ((D + C) \<cdot> \<mu> \<cdot> \<rho>)) (inv_renaming' \<rho> \<odot> \<sigma> \<odot> \<delta>)"
+
+  show ?thesis
+    unfolding regular_state_def
+  proof (intro conjI exI)
+    show "sound_state N S2"
+      by (rule resolve_sound_state[OF step sound_S1])
+  next
+    show "S2 = (\<Gamma>, U, Some ((D + C) \<cdot> \<mu> \<cdot> \<rho>, ?\<gamma>))"
+      using resolveI by simp
+  next
+    from sound_S1 have "sound_trail N U \<Gamma>"
+      using resolveI by (simp add: sound_state_def)
+    then obtain CC :: "('f, 'v) term clause" and \<rho>\<^sub>C\<^sub>C :: "('f, 'v) subst" where
+      CC_in: "CC \<in> N \<union> U" and
+      "is_renaming \<rho>\<^sub>C\<^sub>C" and
+      "add_mset L C = CC \<cdot> \<rho>\<^sub>C\<^sub>C"
+      using resolveI unfolding sound_trail.simps[of N U \<Gamma>]
+      by (auto simp: trail_propagate_def)
+
+    show "trail_almost_no_conflict
+      (N \<union> U \<union> (case Some ((D + C) \<cdot> \<mu> \<cdot> \<rho>, ?\<gamma>) of None \<Rightarrow> {} | Some (C, \<gamma>) \<Rightarrow> {C})) \<Gamma>"
+      apply simp
+      using tr_almost_no_conf
+      apply (simp add: trail_almost_no_conflict_def)
+      unfolding trail_no_conflict_def
+      apply (erule contrapos_nn)
+      apply (elim exE conjE)
+        unfolding insert_iff
+        apply (erule disjE)
+        subgoal for E \<gamma>
+          apply (rule exI[of _ "add_mset L' D"])
+          apply simp
+          apply (rule exI[of _ "\<mu> \<odot> \<rho> \<odot> \<gamma>"])
+          apply simp
+          unfolding trail_false_cls_def
+          apply simp
+          sorry
+        subgoal for C \<gamma>
+          by blast
+        done
+  qed
+qed
+
+lemma trail_backtrack_decide_Suc_level[simp]:
+  "trail_backtrack (trail_decide \<Gamma> L) (Suc (trail_level \<Gamma>)) = trail_decide \<Gamma> L"
+  by (smt (verit, best) id_def n_not_Suc_n trail_backtrack.simps(2) trail_decide_def
+      trail_level.simps(2) trail_level_decide)
+
+lemma finite_Union_iff: "finite (\<Union> S) \<longleftrightarrow> finite S \<and> (\<forall>s \<in> S. finite s)"
+  by (meson Union_upper finite_Union finite_UnionD finite_subset)
+
+lemma trail_no_conflict_if_not_conflict_and_sound:
+  fixes N :: "('f, 'v) term clause set"
+  assumes "sound_state N S1"
+  shows "(\<nexists>S2. conflict N S1 S2) \<Longrightarrow> state_conflict S1 = None \<Longrightarrow>
+    trail_no_conflict (N \<union> state_learned S1) (state_trail S1)"
+proof (erule contrapos_np)
+  assume "state_conflict S1 = None"
+  then obtain \<Gamma> :: "('f, 'v) trail" and U :: "('f, 'v) term clause set" where
+    S1_def: "S1 = (\<Gamma>, U, None)"
+    by (metis prod.collapse state_conflict_def)
+  with \<open>sound_state N S1\<close> have "finite N" and "finite U"
+    unfolding sound_state_def by simp_all
+
+  assume "\<not> trail_no_conflict (N \<union> state_learned S1) (state_trail S1)"
+  then obtain C :: "('f, 'v) term clause" and \<gamma> :: "('f, 'v) subst" where
+    "C \<in> N \<union> U" and "trail_false_cls \<Gamma> (C \<cdot> \<gamma>)"
+    by (auto simp: S1_def trail_no_conflict_def)
+
+  define \<rho>_vars :: "'v \<Rightarrow> 'v" where
+    "\<rho>_vars = renaming_vars (\<Union> (vars_cls ` (N \<union> U \<union> clss_of_trail \<Gamma>)))"
+
+  have "inj \<rho>_vars"
+    unfolding \<rho>_vars_def
+  proof (rule inj_renaming)
+    show "finite (\<Union> (vars_cls ` (N \<union> U \<union> clss_of_trail \<Gamma>)))"
+      using \<open>finite N\<close> \<open>finite U\<close> by simp
+  qed
+
+  define C' :: "('f, 'v) term clause" where
+    "C' = C \<cdot> (Var \<circ> \<rho>_vars)"
+  define \<gamma>' :: "('f, 'v) subst" where
+    "\<gamma>' = (\<lambda>x. if x \<in> \<rho>_vars ` vars_cls C then \<gamma> (the_inv \<rho>_vars x) else Var x)"
+
+  have "C \<cdot> ((Var \<circ> \<rho>_vars) \<odot> \<gamma>') = C \<cdot> \<gamma>"
+    by (rule same_on_vars_clause) (simp add: subst_compose_def \<gamma>'_def \<open>inj \<rho>_vars\<close> the_inv_f_f)
+  hence "C' \<cdot> \<gamma>' = C \<cdot> \<gamma>"
+    unfolding C'_def by simp
+
+  show "\<exists>S2. conflict N S1 S2"
+  proof (rule exI)
+    show "conflict N S1 (\<Gamma>, U, Some (C', \<gamma>'))"
+      unfolding S1_def
+    proof (rule conflictI)
+      show "C \<in> N \<union> U"
+        by (rule \<open>C \<in> N \<union> U\<close>)
+    next
+      show "C' = rename_clause (N \<union> U \<union> clss_of_trail \<Gamma>) C"
+        unfolding C'_def rename_clause_def \<rho>_vars_def by (rule refl)
+    next
+      have "renaming_vars (\<Union>(vars_cls ` (N \<union> U \<union> clss_of_trail \<Gamma>))) x \<noteq> x" for x
+        by (simp add: \<open>finite N\<close> \<open>finite U\<close> renaming_all)
+      hence "renaming_wrt (N \<union> U \<union> clss_of_trail \<Gamma>) x \<noteq> Var x" for x
+        by simp
+      hence "subst_domain (Var \<circ> \<rho>_vars) = UNIV"
+        unfolding \<rho>_vars_def subst_domain_def by simp
+      hence "vars_cls (C \<cdot> (Var \<circ> \<rho>_vars)) = \<rho>_vars ` vars_cls C"
+        unfolding vars_subst_cls_eq by auto
+      thus "subst_domain \<gamma>' \<subseteq> vars_cls C'"
+        unfolding \<gamma>'_def C'_def by (smt (verit, best) mem_Collect_eq subsetI subst_domain_def)
+    next
+      from \<open>sound_state N S1\<close> have "sound_trail N U \<Gamma>"
+        unfolding sound_state_def S1_def by simp
+      hence "\<forall>L \<in> fst ` set \<Gamma>. is_ground_lit L"
+        by (rule ball_ground_lit_if_sound_trail)
+      hence "is_ground_cls (C \<cdot> \<gamma>)"
+        unfolding is_ground_cls_def
+        apply (intro allI impI)
+        apply (drule \<open>trail_false_cls \<Gamma> (C \<cdot> \<gamma>)\<close>[unfolded trail_false_cls_def, rule_format])
+        unfolding trail_false_lit_def is_ground_lit_def
+        by (metis atm_of_uminus)
+      thus "is_ground_cls (C' \<cdot> \<gamma>')"
+        using \<open>C' \<cdot> \<gamma>' = C \<cdot> \<gamma>\<close> by simp
+    next
+      show "trail_false_cls \<Gamma> (C' \<cdot> \<gamma>')"
+        using \<open>trail_false_cls \<Gamma> (C \<cdot> \<gamma>)\<close> \<open>C' \<cdot> \<gamma>' = C \<cdot> \<gamma>\<close> by simp
+    qed
+  qed
+qed
+
+
+
+lemma decide_regular_state:
+  assumes step: "decide N S1 S2" and no_conflict: "\<nexists>S3. conflict N S2 S3" and "regular_state N S1"
+  shows "regular_state N S2"
+  using step
+proof (cases N S1 S2 rule: decide.cases)
+  case (decideI L \<Gamma> U)
+  with \<open>regular_state N S1\<close> have
+    sound_S1: "sound_state N S1" and
+    tr_almost_no_conf: "trail_almost_no_conflict (N \<union> U) \<Gamma>"
+    by (simp_all add: regular_state_def)
+
+  have sound_S2: "sound_state N S2"
+      by (rule decide_sound_state[OF step sound_S1])
+
+  show ?thesis
+    unfolding regular_state_def
+  proof (intro conjI exI)
+    show "sound_state N S2"
+      by (rule sound_S2)
+  next
+    show "S2 = (trail_decide \<Gamma> L, U, None)"
+      using decideI by simp
+  next
+    have "trail_no_conflict (N \<union> state_learned S2) (state_trail S2)"
+      by (rule trail_no_conflict_if_not_conflict_and_sound[OF sound_S2 no_conflict])
+        (use decideI in simp)
+    thus "trail_almost_no_conflict
+      (N \<union> U \<union> (case None of None \<Rightarrow> {} | Some (C, \<gamma>) \<Rightarrow> {C})) (trail_decide \<Gamma> L)"
+      using decideI by (simp add: trail_almost_no_conflict_if_trail_no_conflict)
+  qed
+qed
+
+lemma
+  assumes
+    sound_S1: "sound_state N S1" and
+    regular_step: "regular_scl N S1 S2" and
+    regular_S1: "regular_state N S1"
+  shows "regular_state N S2"
+  using regular_step unfolding regular_scl_def
+proof (elim disjE conjE)
+  show "conflict N S1 S2 \<Longrightarrow> ?thesis"
+    by (rule conflict_regular_state[OF _ regular_S1])
+next
+  from regular_S1 have
+    sound_S1: "sound_state N S1" and
+    almost_no_conf_S1: "trail_almost_no_conflict
+       (N \<union> state_learned S1 \<union> (case state_conflict S1 of None \<Rightarrow> {} | Some (C, \<gamma>) \<Rightarrow> {C}))
+       (state_trail S1)"
+    unfolding regular_state_def by auto
+  from regular_step sound_S1 have sound_S2: "sound_state N S2"
+    by (rule regular_scl_sound_state)
+
+  assume "\<not> conflict N S1 S2" and "reasonable_scl N S1 S2"
+  thus ?thesis
+    unfolding reasonable_scl_def scl_def
+  proof (elim disjE conjE)
+    show "propagate N S1 S2 \<Longrightarrow> ?thesis"
+      by (rule propagate_regular_state[OF _ regular_S1])
+  next
+    assume "decide N S1 S2" and "decide N S1 S2 \<longrightarrow> \<not> Ex (conflict N S2)"
+    thus ?thesis
+      using decide_regular_state[OF _ _ regular_S1] by simp
+  next
+    assume "\<not> conflict N S1 S2" and "conflict N S1 S2"
+    hence False by simp
+    thus ?thesis ..
+  next
+    show "skip N S1 S2 \<Longrightarrow> ?thesis"
+      by (rule skip_regular_state[OF _ regular_S1])
+  next
+    show "factorize N S1 S2 \<Longrightarrow> ?thesis"
+      by (rule factorize_regular_state[OF _ regular_S1])
+  next
+    show "resolve N S1 S2 \<Longrightarrow> ?thesis"
+      using tr_almost_no_conf by (auto simp add: resolve.simps trail_almost_no_conflict_def)
+  next
+    show "backtrack N S1 S2 \<Longrightarrow> ?thesis"
+      apply (erule backtrack.cases)
+      using almost_no_conf_S1
+      apply (simp add: regular_state_def)
+      using trail_no_conflict_suffixI[OF trail_backtrack_suffix]
+      
+      find_theorems "suffix (trail_backtrack _ _) _"
+      
+      
+
+lemma
+  assumes
+    fin_N: "finite N" and disj_vars_N: "disjoint_vars_set N" and
+    regular_run: "(regular_scl N)\<^sup>*\<^sup>* initial_state S0" and
+    regular_step: "backtrack N S0 S1"
+  shows "\<not> conflict N S1 S2"
+  using regular_run regular_step
+  thm converse_rtranclp_induct
+proof (induction arbitrary: rule: converse_rtranclp_induct)
+  case base
+  hence False by (simp add: backtrack.simps)
+  thus ?case ..
+next
+  case (step S0 S0')
+  then show ?case
+    
+    sorry
+qed
+
+
+lemma propagate_or_backtrack_before_regular_conflict:
+  assumes
+    fin_N: "finite N" and disj_vars_N: "disjoint_vars_set N" and
+    regular_run: "(regular_scl N)\<^sup>*\<^sup>* initial_state S0" and
+    regular_step: "regular_scl N S0 S1" and
+    conflict: "conflict N S1 S2"
+  shows "propagate N S0 S1 \<or> backtrack N S0 S1"
+proof -
+  from conflict obtain \<Gamma> U C \<gamma> where
+    S1_def: "S1 = (\<Gamma>, U, None)" and
+    S2_def: "S2 = (\<Gamma>, U, Some (C, \<gamma>))"
+    unfolding conflict.simps by auto
+
+  with regular_step have "\<not> conflict N S0 S1" and "reasonable_scl N S0 S1"
+    unfolding regular_scl_def by (simp_all add: conflict.simps)
+
+  with conflict have "scl N S0 S1" and "\<not> decide N S0 S1"
+    unfolding reasonable_scl_def by blast+
+
+  thus ?thesis
+    unfolding scl_def
+    by (simp add: S1_def skip.simps conflict.simps factorize.simps resolve.simps)
+qed
+
+(* lemma
+  assumes
+    fin_N: "finite N" and disj_vars_N: "disjoint_vars_set N" and
+    regular_run: "(regular_scl N)\<^sup>*\<^sup>* initial_state S1" and
+    conflict: "conflict N S1 S2"
+  shows "{#} \<in> N \<or> (\<exists>S0. (regular_scl N)\<^sup>*\<^sup>* initial_state S0 \<and> propagate N S0 S1)" *)
+  
+
+lemma
+  assumes
+    fin_N: "finite N" and disj_vars_N: "disjoint_vars_set N" and
+    regular_run: "(regular_scl N)\<^sup>*\<^sup>* initial_state S0" and
+    conflict: "conflict N S0 S1" and
+    resolution: "(\<lambda>S S'. skip N S S' \<or> factorize N S S' \<or> resolve N S S')\<^sup>+\<^sup>+ S1 Sn" and
+    backtrack: "backtrack N Sn Sn'" and
+    "transp lt" and
+    total_on_ground_lt: "Restricted_Predicates.total_on lt {L. is_ground_lit L}"
+  shows "(regular_scl N)\<^sup>*\<^sup>* initial_state Sn' \<and>
+    (\<exists>C \<gamma>. state_conflict Sn = Some (C, \<gamma>) \<and>
+      \<not> redundant (multp (trail_less_ex lt (map fst (state_trail S1)))) (N \<union> U) C)"
+proof -
+  from regular_run conflict have "(regular_scl N)\<^sup>*\<^sup>* initial_state S1"
+    by (meson regular_scl_def rtranclp.simps)
+  also from resolution have "(regular_scl N)\<^sup>*\<^sup>* ... Sn"
+    using regular_run_if_skip_factorize_resolve_run tranclp_into_rtranclp by fast
+  also from backtrack have "(regular_scl N)\<^sup>*\<^sup>* ... Sn'"
+    by (auto simp add: scl_def reasonable_scl_def regular_scl_def backtrack_well_defined)
+  finally have "(regular_scl N)\<^sup>*\<^sup>* initial_state Sn'" by assumption
+
+  from conflict obtain C1 \<gamma>1 where conflict_S1: "state_conflict S1 = Some (C1, \<gamma>1)"
+    by (smt (verit, best) conflict.simps state_conflict_simp)
+  then obtain Cn \<gamma>n where conflict_Sn: "state_conflict Sn = Some (Cn, \<gamma>n)"
+    by (smt (verit) backtrack.simps backtrack state_conflict_simp)
+
+  from fin_N disj_vars_N have "sound_state N initial_state"
+    by (rule sound_initial_state)
+  with regular_run have "sound_state N S0"
+    by (simp add: regular_run_sound_state)
+  with conflict have sound_S1: "sound_state N S1"
+    by (simp add: conflict_sound_state)
+  with resolution have sound_Sn: "sound_state N Sn"
+    by (induction rule: tranclp_induct)
+      (auto intro: skip_sound_state factorize_sound_state resolve_sound_state)
+
+  from conflict_Sn sound_Sn have "N \<TTurnstile>\<G>e {Cn}" and
+    trail_Sn_false_Cn_\<gamma>n: "trail_false_cls (state_trail Sn) (Cn \<cdot> \<gamma>n)"
+    by (auto simp add: sound_state_def)
+
+  from conflict_S1 sound_S1 have trail_S1_false_C1_\<gamma>1: "trail_false_cls (state_trail S1) (C1 \<cdot> \<gamma>1)"
+    by (auto simp add: sound_state_def)
+
+  from resolution have "suffix (state_trail Sn) (state_trail S1) \<and>
+    (\<exists>Cn \<gamma>n. state_conflict Sn = Some (Cn, \<gamma>n) \<and> trail_false_cls (state_trail S1) (Cn \<cdot> \<gamma>n))"
+  proof (induction Sn rule: tranclp_induct)
+    case (base S2)
+    thus ?case
+    proof (elim disjE)
+      assume "skip N S1 S2"
+      thus ?thesis
+        using trail_false_conflict_after_skip[OF conflict_S1 trail_S1_false_C1_\<gamma>1]
+        by (smt (verit) skip.simps state_trail_simp suffix_trail_propagate)
+    next
+      assume "factorize N S1 S2"
+      moreover with sound_S1 have "sound_state N S2"
+        by (auto intro: factorize_sound_state)
+      ultimately show ?thesis
+        by (cases N S1 S2 rule: factorize.cases) (simp add: sound_state_def)
+    next
+      assume "resolve N S1 S2"
+      moreover with sound_S1 have "sound_state N S2"
+        by (auto intro: resolve_sound_state)
+      ultimately show ?thesis
+        by (cases N S1 S2 rule: resolve.cases) (simp add: sound_state_def)
+    qed
+  next
+    case (step Sm Sm')
+    from step.hyps(2) have "suffix (state_trail Sm') (state_trail Sm)"
+      by (auto dest: strict_suffix_trail_if_skip eq_trail_if_factorize eq_trail_if_resolve)
+    with step.IH have "suffix (state_trail Sm') (state_trail S1)"
+      by force
+
+    from step.hyps(1) sound_S1 have sound_Sm: "sound_state N Sm"
+      by (induction rule: tranclp_induct)
+        (auto intro: skip_sound_state factorize_sound_state resolve_sound_state)
+
+    from step.IH obtain Cm \<gamma>m where
+      conflict_Sm: "state_conflict Sm = Some (Cm, \<gamma>m)" and
+      trail_false_Cm_\<gamma>m: "trail_false_cls (state_trail S1) (Cm \<cdot> \<gamma>m)"
+      using step.prems step.hyps(2) \<open>suffix (state_trail Sm') (state_trail Sm)\<close>
+      by auto
+
+    from step.hyps(2) show ?case
+    proof (elim disjE)
+      assume "skip N Sm Sm'"
+      thus ?thesis
+        using \<open>suffix (state_trail Sm') (state_trail S1)\<close>
+        using trail_false_conflict_after_skip trail_false_Cm_\<gamma>m conflict_Sm
+        by (smt (verit) skip.cases state_conflict_simp)
+    next
+      assume "factorize N Sm Sm'"
+      thus ?thesis
+      proof (cases N Sm Sm' rule: factorize.cases)
+        case (factorizeI L \<sigma> L' \<mu> \<sigma>' D \<Gamma> U)
+        with conflict_Sm have Cm_def: "Cm = D + {#L, L'#}" and \<gamma>m_def: "\<gamma>m = \<sigma>"
+          by simp_all
+        with factorizeI(3,4) have "trail_false_cls (state_trail S1) ((D + {#L#}) \<cdot> \<mu> \<cdot> \<sigma>)"
+          using trail_false_Cm_\<gamma>m trail_false_cls_subst_mgu_before_grounding
+          by (smt (verit, best) CollectI mgu_sound prod.sel singletonD atm_of_subst_lit
+              unifiers_def)
+        with factorizeI(5) have "trail_false_cls (state_trail S1) ((D + {#L#}) \<cdot> \<mu> \<cdot> \<sigma>')"
+          by (metis subsetI subst_cls_restrict_subst_idem)
+        with factorizeI(2) show ?thesis
+          using \<open>suffix (state_trail Sm') (state_trail S1)\<close>
+          using state_conflict_simp by blast
+      qed
+    next
+      assume "resolve N Sm Sm'"
+      thus ?thesis
+      proof (cases N Sm Sm' rule: resolve.cases)
+        case (resolveI \<Gamma> \<Gamma>' L C \<delta> D \<sigma> \<rho> U L' \<mu>)
+        have "is_renaming (renaming_wrt (N \<union> U \<union> clss_of_trail \<Gamma> \<union> {D + {#L'#}}))"
+          apply (rule is_renaming_renaming_wrt)
+          using resolveI
+          by (smt (verit, best) finite.emptyI finite.insertI finite_UnI finite_clss_of_trail
+              sound_Sm sound_state_def state_learned_simp)
+        with resolveI have is_renaming_\<rho>: "is_renaming \<rho>"
+          by simp
+
+        from resolveI conflict_Sm have Cm_def: "Cm = D + {#L'#}" and \<gamma>m_def: "\<gamma>m = \<sigma>"
+          by simp_all
+        hence tr_false_D_L'_\<sigma>: "trail_false_cls (state_trail S1) ((D + {#L'#}) \<cdot> \<sigma>)"
+          using trail_false_Cm_\<gamma>m by simp
+
+        from resolveI sound_Sm have
+          "disjoint_vars_set (N \<union> U \<union> clss_of_trail \<Gamma>)" and
+          disj_N_U_\<Gamma>_D_L': "\<forall>C \<in> N \<union> U \<union> clss_of_trail \<Gamma>. disjoint_vars (D + {#L'#}) C" and
+          "is_ground_cls ((D + {#L'#}) \<cdot> \<sigma>)" and
+          dom_\<sigma>: "subst_domain \<sigma> \<subseteq> vars_cls (D + {#L'#})" and
+          "sound_trail N U \<Gamma>"
+          unfolding sound_state_def by simp_all
+
+        have "vars_cls (D + {#L'#}) \<inter> vars_cls (C + {#L#}) = {}"
+          apply(rule disj_N_U_\<Gamma>_D_L'[unfolded disjoint_vars_iff_inter_empty,
+                rule_format, of "C + {#L#}"])
+          by (simp add: resolveI(3))
+
+        from resolveI(6) have "atm_of (L \<cdot>l \<delta>) = atm_of (L' \<cdot>l \<sigma>)" by simp
+        hence "(atm_of L) \<cdot>a \<delta> = (atm_of L') \<cdot>a \<sigma>" by simp
+
+        have \<sigma>_\<delta>_in_unif: "\<sigma> \<odot> \<delta> \<in> unifiers {(atm_of L, atm_of L')}"
+        proof (rule subst_comp_in_unifiersI')
+          show "atm_of L \<cdot>a \<delta> = atm_of L' \<cdot>a \<sigma>"
+            using resolveI(6) by (metis atm_of_eq_uminus_if_lit_eq atm_of_subst_lit)
+        next
+          show "vars_lit L \<inter> subst_domain \<sigma> = {}"
+            using dom_\<sigma> \<open>vars_cls (D + {#L'#}) \<inter> vars_cls (C + {#L#}) = {}\<close> by fastforce
+        next
+          have "subst_domain \<delta> \<subseteq> vars_cls C \<union> vars_lit L"
+            using \<open>sound_trail N U \<Gamma>\<close>
+            unfolding sound_trail.simps[of N U \<Gamma>]
+            unfolding resolveI(3)
+            by (simp add: trail_propagate_def)
+          then show "vars_lit L' \<inter> subst_domain \<delta> = {}"
+            using \<open>vars_cls (D + {#L'#}) \<inter> vars_cls (C + {#L#}) = {}\<close> by auto
+        next
+          have "range_vars \<sigma> = {}"
+            unfolding range_vars_def UNION_empty_conv subst_range.simps
+            using dom_\<sigma> \<open>is_ground_cls ((D + {#L'#}) \<cdot> \<sigma>)\<close> is_ground_cls_is_ground_on_var
+              is_ground_atm_iff_vars_empty
+            by fast
+          thus "range_vars \<sigma> \<inter> subst_domain \<delta> = {}"
+            by simp
+        qed
+
+        from resolveI \<open>sound_trail N U \<Gamma>\<close> have "trail_false_cls \<Gamma>' (C \<cdot> \<delta>)"
+          by (auto simp: trail_propagate_def elim: sound_trail.cases)
+
+        from resolveI have "suffix \<Gamma>' (state_trail S1)"
+          using \<open>suffix (state_trail Sm') (state_trail S1)\<close>
+          by (metis (no_types, lifting) state_trail_simp suffix_order.trans suffix_trail_propagate)
+
+        have "trail_false_cls (state_trail S1) ((D + C) \<cdot> \<mu> \<cdot> \<sigma> \<cdot> \<delta>)"
+          using trail_false_cls_plus_subst_mgu_before_groundings[
+              of "state_trail S1" D L' \<sigma> _ C \<delta> L \<mu>, OF tr_false_D_L'_\<sigma> \<open>trail_false_cls \<Gamma>' (C \<cdot> \<delta>)\<close>
+                \<open>suffix \<Gamma>' (state_trail S1)\<close>
+                \<open>is_ground_cls ((D + {#L'#}) \<cdot> \<sigma>)\<close>
+                \<open>vars_cls (D + {#L'#}) \<inter> vars_cls (C + {#L#}) = {}\<close>
+                \<open>subst_domain \<sigma> \<subseteq> vars_cls (D + {#L'#})\<close>
+                mgu_sound[OF resolveI(7)] \<sigma>_\<delta>_in_unif]
+          by assumption
+        then have "trail_false_cls (state_trail S1) ((D + C) \<cdot> \<mu> \<cdot> \<rho> \<cdot>
+          restrict_subst (vars_cls ((D + C) \<cdot> \<mu> \<cdot> \<rho>)) (inv_renaming' \<rho> \<odot> \<sigma> \<odot> \<delta>))"
+          unfolding subst_cls_restrict_subst_idem[OF subset_refl]
+          unfolding subst_cls_comp_subst subst_cls_renaming_inv_renaming_idem[OF is_renaming_\<rho>]
+          by assumption
+        then show ?thesis
+          using \<open>suffix (state_trail Sm') (state_trail S1)\<close>
+          using resolveI by simp
+      qed
+    qed
+  qed
+
+  then obtain Cn \<gamma>n where
+    "suffix (state_trail Sn) (state_trail S1)" and
+    conflict_Sn: "state_conflict Sn = Some (Cn, \<gamma>n)" and
+    "trail_false_cls (state_trail S1) (Cn \<cdot> \<gamma>n)"
+    by auto
+
+  moreover have "\<not> redundant (multp (trail_less_ex lt (map fst (state_trail S1)))) (N \<union> U) Cn"
+  proof (rule notI)
+    assume "redundant (multp (trail_less_ex lt (map fst (state_trail S1)))) (N \<union> U) Cn"
+    moreover from sound_Sn conflict_Sn have "Cn \<cdot> \<gamma>n \<in> grounding_of_cls Cn"
+      unfolding sound_state_def
+      using grounding_of_cls_ground grounding_of_subst_cls_subset 
+      by fastforce
+    ultimately have gr_red_Cn_\<gamma>n: "ground_redundant
+      (multp (trail_less_ex lt (map fst (state_trail S1))))
+      (grounding_of_clss (N \<union> U)) (Cn \<cdot> \<gamma>n)"
+      by (simp add: redundant_def)
+
+    define S where
+      "S = {D \<in> grounding_of_clss (N \<union> U).
+        (multp (trail_less_ex lt (map fst (state_trail S1))))\<^sup>=\<^sup>= D (Cn \<cdot> \<gamma>n)}"
+
+    from gr_red_Cn_\<gamma>n have "S \<TTurnstile>e {Cn \<cdot> \<gamma>n}"
+      unfolding ground_redundant_def S_def by simp
+
+    from sound_S1 have "sound_trail N (state_learned S1) (state_trail S1)"
+      by (auto simp add: sound_state_def)
+
+    have "\<forall>L\<in>#Cn \<cdot> \<gamma>n. trail_defined_lit (state_trail S1) L"
+      using \<open>trail_false_cls (state_trail S1) (Cn \<cdot> \<gamma>n)\<close> trail_defined_lit_iff_true_or_false
+        trail_false_cls_def by blast
+
+    have "\<not> trail_interp (state_trail S1) \<TTurnstile>s {Cn \<cdot> \<gamma>n}"
+      apply (rule notI)
+      using \<open>trail_false_cls (state_trail S1) (Cn \<cdot> \<gamma>n)\<close>
+      apply simp
+      unfolding trail_true_cls_iff_trail_interp_entails[OF
+          \<open>sound_trail N (state_learned S1) (state_trail S1)\<close>
+          \<open>\<forall>L\<in>#Cn \<cdot> \<gamma>n. trail_defined_lit (state_trail S1) L\<close>, symmetric]
+      using not_trail_true_and_false_cls[OF \<open>sound_trail N (state_learned S1) (state_trail S1)\<close>]
+      by simp
+
+    hence "\<not> trail_interp (state_trail S1) \<TTurnstile>s S"
+      using \<open>S \<TTurnstile>e {Cn \<cdot> \<gamma>n}\<close>[rule_format, of "trail_interp (state_trail S1)"]
+      by argo
+
+    then obtain D where "D \<in> S" and "\<not> trail_interp (state_trail S1) \<TTurnstile> D"
+      by (auto simp: true_clss_def)
+
+    moreover have "trail_defined_cls (state_trail S1) D"
+    proof -
+      have "trail_defined_cls (state_trail S1) (Cn \<cdot> \<gamma>n)"
+        using \<open>\<forall>L\<in>#Cn \<cdot> \<gamma>n. trail_defined_lit (state_trail S1) L\<close> trail_defined_cls_def by blast
+
+      from \<open>D \<in> S\<close> have
+        D_in: "D \<in> grounding_of_clss (N \<union> U)" and
+        "(multp (trail_less_ex lt (map fst (state_trail S1))))\<^sup>=\<^sup>= D (Cn \<cdot> \<gamma>n)"
+        unfolding S_def by simp_all
+      then show "trail_defined_cls (state_trail S1) D"
+        unfolding Lattices.sup_apply Boolean_Algebras.sup_bool_def
+      proof (elim disjE)
+        assume multp_D_Cn_\<gamma>n: "multp (trail_less_ex lt (map fst (state_trail S1))) D (Cn \<cdot> \<gamma>n)"
+        show "trail_defined_cls (state_trail S1) D"
+        proof (rule trail_defined_cls_if_lt_defined)
+          show "sound_trail N (state_learned S1) (state_trail S1)"
+            by (rule \<open>sound_trail N (state_learned S1) (state_trail S1)\<close>)
+        next
+          show "multp (trail_less_ex lt (map fst (state_trail S1))) D (Cn \<cdot> \<gamma>n)"
+            by (rule multp_D_Cn_\<gamma>n)
+        next
+          show "trail_defined_cls (state_trail S1) (Cn \<cdot> \<gamma>n)"
+            by (rule \<open>trail_defined_cls (state_trail S1) (Cn \<cdot> \<gamma>n)\<close>)
+        next
+          show "transp lt"
+            by (rule \<open>transp lt\<close>)
+        next
+          have "is_ground_cls D"
+            using D_in by (simp add: grounding_ground)
+          moreover have "is_ground_cls (Cn \<cdot> \<gamma>n)"
+            using \<open>Cn \<cdot> \<gamma>n \<in> grounding_of_cls Cn\<close> is_ground_cls_if_in_grounding_of_cls by blast
+          ultimately have "set_mset D \<union> set_mset (Cn \<cdot> \<gamma>n) \<subseteq> {L. is_ground_lit L}"
+            using is_ground_cls_imp_is_ground_lit by auto
+          thus "Restricted_Predicates.total_on lt (set_mset D \<union> set_mset (Cn \<cdot> \<gamma>n))"
+            using total_on_ground_lt
+            by (metis le_iff_sup total_on_unionD1)
+        qed
+      next
+        assume "D = Cn \<cdot> \<gamma>n"
+        then show "trail_defined_cls (state_trail S1) D"
+          using \<open>trail_defined_cls (state_trail S1) (Cn \<cdot> \<gamma>n)\<close> by simp
+      qed    
+    qed
+
+    then have "trail_false_cls (state_trail S1) D"
+      using \<open>\<not> trail_interp (state_trail S1) \<TTurnstile> D\<close>
+      by (meson \<open>sound_trail N (state_learned S1) (state_trail S1)\<close> trail_defined_cls_def
+          trail_defined_lit_iff_true_or_false trail_false_cls_def
+          trail_interp_cls_if_sound_and_trail_true trail_true_cls_def)
+
+    from conflict obtain S
+
+    from conflict obtain L C \<gamma> where "state_trail S1 = trail_propagate (state_trail S0) L C \<gamma>"
+      apply (elim conflict.cases)
+
+    thus False
+      sorry
+  qed
+
+  ultimately show ?thesis
+    using \<open>(regular_scl N)\<^sup>*\<^sup>* initial_state Sn'\<close>
+    by simp
+  oops
+    
 
 end
 
